Template proofs for BST

concurrency/bst_template.c
@@ -6,10 +6,11 @@
 //
 
 
-#include <stddef.h>
+
 #include <stdio.h>
 /* #include <stdlib.h> */
 #include "threads.h"
+
 
 extern void *malloc (size_t n);
 extern void free(void *p);
@@ -19,7 +20,6 @@ typedef struct tree {int key; void *value; struct tree_t *left, *right;} tree;
 typedef struct tree_t {tree *t; lock_t *lock;} tree_t;
 
 typedef struct tree_t **treebox;
-lock_t thread_lock;
 treebox tb;
 
 
@@ -33,11 +33,11 @@ treebox treebox_new(void) {
     treebox p = (treebox) surely_malloc(sizeof (*p));
     tree_t *newt = (tree_t *) surely_malloc(sizeof(tree_t));
     *p = newt;
-    lock_t *l = (lock_t *) surely_malloc(sizeof(lock_t));
-    makelock(l);
+    lock_t *l;
+    l = makelock();
     newt->lock = l;
     newt->t = NULL;
-    release2(l);
+    release(l);
     return p;
 }
 
@@ -55,7 +55,7 @@ void tree_free(struct tree_t *tgp) {
         tree_free(pa);
         tree_free(pb);
     }
-    freelock2(l);
+    freelock(l);
     free(l);
     free(tgp);
 }
@@ -65,61 +65,6 @@ void treebox_free(treebox b) {
     tree_free(t);
     free(b);
 }
-
-//Orginal Code
-void insert (treebox t, int x, void *value) {
-    struct tree_t *tgt = *t;
-    struct tree *p;
-    void *l = tgt->lock;
-    acquire(l);
-    for(;;) {
-        p = tgt->t;
-        if (p==NULL) {
-            tree_t *p1 = (struct tree_t *) surely_malloc (sizeof *tgt);
-            tree_t *p2 = (struct tree_t *) surely_malloc (sizeof *tgt);
-            p1 ->t = NULL;
-            p2 ->t = NULL;
-            lock_t *l1 = (lock_t *) surely_malloc(sizeof(lock_t));
-            makelock(l1);
-            p1->lock = l1;
-            release2(l1);
-            lock_t *l2 = (lock_t *) surely_malloc(sizeof(lock_t));
-            makelock(l2);
-            p2->lock = l2;
-            release2(l2);
-            p = (struct tree *) surely_malloc (sizeof *p);
-            tgt->t = p;
-            p->key=x; p->value=value; p->left=p1; p->right=p2;
-            
-            //  printf ("%d %s\n", p->key, p->value);
-            release2(l);
-            return;
-        } else {
-            int y = p->key;
-            if (x<y){
-                tgt = p->left;
-                printf("Left - x = %d, y = %d\n", x, p->key);
-                void *l_old = l;
-                l = tgt->lock;
-                acquire(l);
-                release2(l_old);
-            } else if (y<x){
-                tgt = p->right;
-                printf("Right - x = %d, y = %d\n", x, p->key);
-                void *l_old = l;
-                l = tgt->lock;
-                acquire(l);
-                release2(l_old);
-            }else {
-                p->value=value;
-                printf ("Exclude %d %s\n", p->key, p->value);
-                release2(l);
-                return;
-            }
-        }
-    }
-}
-
 
 //Template style
 
@@ -160,7 +105,7 @@ int traverse(pn *pn, int x, void *value) {
             }
             else{
                 acquire(pn->n->lock);
-                release2(pn->p->lock);
+                release(pn->p->lock);
             }
         }
     }
@@ -172,14 +117,14 @@ void insertOp(pn *pn, int x, void *value){
     tree_t *p2 = (struct tree_t *) surely_malloc (sizeof *(pn->p));
     p1->t = NULL;
     p2->t = NULL;
-    lock_t *l1 = (lock_t *) surely_malloc(sizeof(lock_t));
-    makelock(l1);
+    lock_t *l1;
+    l1 = makelock();
     p1->lock = l1;
-    release2(l1);
-    lock_t *l2 = (lock_t *) surely_malloc(sizeof(lock_t));
-    makelock(l2);
+    release(l1);
+    lock_t *l2;
+    l2 = makelock();
     p2->lock = l2;
-    release2(l2);
+    release(l2);
     pn->p->t = (struct tree *) surely_malloc (sizeof *(pn->p->t));
     pn->p->t->key = x;
     pn->p->t->value = value;
@@ -201,9 +146,10 @@ void insert2 (treebox t, int x, void *value) {
         insertOp(pn, x, value);
     }
     //release2(pn->p->lock);
-    release2(pn->n->lock);
+    release(pn->n->lock);
     free(pn);
 }
+
 
 //Traverse
 void Inorder(struct tree_t *p){
@@ -215,7 +161,6 @@ void Inorder(struct tree_t *p){
 }
 
 void traverseInorder (treebox t){
-    struct tree *p;
     struct tree_t *tgt;
     tgt = *t;
     Inorder(tgt);
@@ -236,42 +181,42 @@ void *lookup (treebox t, int x) {
       l = tgt->lock;
       acquire(l);
       p=tgt->t;
-      release2(l_old);
+      release(l_old);
     }else if (y<x){
       tgt=p->right;
       void *l_old = l;
       l = tgt->lock;
       acquire(l);
       p=tgt->t;
-      release2(l_old);
+      release(l_old);
     }else {
       v = p->value;
-      release2(l);
+      release(l);
       return v;
     }
   }
-  release2(l);
+  release(l);
   return NULL;
 }
 
 
 
 void *thread_func(void *args) {
-    lock_t *l = &thread_lock;
+    lock_t *l = (lock_t*)args;
     
     // insert at key 1
-    //insert2(tb,6,"ONE_FROM_THREAD");
-    //insert2(tb,4,"FOUR");
+    insert2(tb,6,"ONE_FROM_THREAD");
+    insert2(tb,4,"FOUR");
     //   insert(tb,5,"FIVE");
     
-    release2((void*)l);
+    release((void*)l);
     return (void *)NULL;
 }
 
 
 int main (void) {
     tb = treebox_new();
-    lock_t *t_lock = &thread_lock;
+    lock_t *t_lock ;
     insert2(tb,3,"three");
     insert2(tb,1,"One");
     insert2(tb,4,"four");
@@ -291,16 +236,17 @@ int main (void) {
     //insert(tb, 6, "six");
     //insert(tb, 5, "five");
     
-    makelock((void*)t_lock);
+    t_lock = makelock();
     /* Spawn */
-    spawn((void *)&thread_func, (void *)NULL);
+    spawn((void *)&thread_func, (void *)t_lock);
     
     //insert at key 1
-    //insert2(tb,1,"ONE");
+    //insert(tb,1,"ONE");
+    //insert(tb,4,"four");
     
     /*JOIN */
     acquire((void*)t_lock);
-    freelock2((void*)t_lock);
+    freelock((void*)t_lock);
     
     // printf ("%d", sizeof (pthread_mutex_t));
     
