concurrency/verif_bst_template.v
@@ -1,11 +1,12 @@
 Require Import VST.concurrency.conclib.
 Require Import VST.floyd.proofauto.
-Require Import VST.floyd.library.
 Require Import VST.atomics.general_locks.
 Require Import Coq.Sets.Ensembles.
 Require Import bst.puretree.
 Require Import bst.bst_template.
 Require Import bst.bst_template_lib.
+Require Import VST.atomics.verif_lock_atomic.
+Require Import VST.floyd.library.
 Import FashNotation.
 
 (*
@@ -29,8 +30,6 @@ We need to write some specs of helper functions: insertOp, traverse and findnext
           {v. ((v = 1 /\ ....) \/ (v = 0 /\  ...)) /\  ... }
 *)
 
-(*change M into t *)
-
 
 Instance gmap_inhabited V : Inhabitant (gmap key V).
 Proof.
@@ -44,17 +43,11 @@ Proof.
   apply Pos_Infinity.
 Defined.
 
-(*
- findnext_spec:
-          {x \in range  /\ ...} findNext(pn *pn, int x, void *value)
-          {v. ((v = 1 /\ ....) \/ (v = 0 /\  ...)) /\  ... }
- *)
-
 Definition tree_rep_1 p (sh :share):=
   EX (tp pa pb vp: val) (xp : Z),
   field_at sh (t_struct_tree_t) [StructField _t] tp p *
   data_at sh t_struct_tree (Vint (Int.repr xp), (vp, (pa, pb))) tp *
-  (!!(is_pointer_or_null pa /\ is_pointer_or_null pb) && emp).
+  (!!(is_pointer_or_null pa /\ is_pointer_or_null pb) && seplog.emp).
 
 Definition pn_rep p n (sh : share) (pn : val) :=
   data_at sh (t_struct_pn) (p, n) pn * tree_rep_1 p sh.
@@ -88,7 +81,8 @@ Definition findnext_spec :=
           PARAMS (b; Vint (Int.repr x); v) GLOBALS (gv)
           SEP (data_at sh (t_struct_pn) (p, n) b;
               field_at sh (t_struct_tree_t) [StructField _t] tp p;
-              data_at sh t_struct_tree (Vint (Int.repr px), (pv, (pa, pb))) tp)
+
+               data_at sh t_struct_tree (Vint (Int.repr px), (pv, (pa, pb))) tp)
   POST [ tint ]
   EX (succ: bool), EX (n' : val),
          PROP (match succ with
@@ -108,45 +102,43 @@ Definition findnext_spec :=
                data_at sh t_struct_tree (Vint (Int.repr px), (pv, (pa, pb))) tp)
              end).
 
-(*
-traverse_spec:
-          < ...  | bst t> traverse(pn *pn, int x, void *value)
-          <v. bst t /\ lock_inv >
-*)
 
 Definition pn_rep_1 (g : gname) (g_root : gname) (sh : share) (pn n: val) :=
   EX (p :val),
   data_at sh (t_struct_pn) (p, n) pn *
   my_half g_root (snd (Share.split gsh1)) (Neg_Infinity, Pos_Infinity, None).
 
-Definition nodebox_rep (g : gname) (g_root : gname) (sh : share) (lock : val) (nb : val) :=
-  EX (np: val), data_at sh (tptr (t_struct_tree_t)) np nb *
-                ltree g g_root sh (fst (Share.split gsh1)) np lock *
-                my_half g_root (snd (Share.split gsh1)) (Neg_Infinity, Pos_Infinity, None).
+Definition nodebox_rep (g : gname) (g_root : gname) (sh : share) (lock : lock_handle) (nb : val) :=
+  EX (np: val), data_at sh (tptr (t_struct_tree_t)) np nb  *
+                 ltree g g_root sh (fst (Share.split gsh1)) np lock * 
+                 my_half g_root (snd (Share.split gsh1)) (Neg_Infinity, Pos_Infinity, None).
 
-Definition node_lock_inv_new sh g p gp lock tp r :=
+Definition node_lock_inv_new sh g p gp (lock : lock_handle) tp r :=
    (field_at Ews t_struct_tree_t (DOT _t) tp p *
-    malloc_token Ews t_struct_tree_t p * in_tree g gp * tree_rep_R tp r.1 r.2 g) *
+    malloc_token Ews t_struct_tree_t p *  in_tree g gp * tree_rep_R tp r.1 r.2 g  ) *
     my_half gp sh r *
-    field_at lsh2 t_struct_tree_t [StructField _lock] lock p *
-    malloc_token Ews tlock lock *
+    field_at lsh2 t_struct_tree_t [StructField _lock] (ptr_of lock) p *
     |> lock_inv lsh2 lock (node_lock_inv sh g p gp lock).
+
+Definition node_lock_inv' sh g p gp lock :=
+  (node_lock_inv_pred sh g p gp (ptr_of lock)) *
+    lock_inv lsh2 lock (node_lock_inv sh g p gp lock).
 
 Program Definition traverse_spec :=
   DECLARE _traverse
-          ATOMIC TYPE (rmaps.ConstType (val * val * share * val  * Z *
+          ATOMIC TYPE (rmaps.ConstType (val * val * share * lock_handle * Z *
                                         val * globals * gname * gname))
-          OBJ M INVS base.empty base.top
+          OBJ M INVS ∅
   WITH  b, n, sh, lock, x, v, gv, g, g_root
   PRE [ tptr t_struct_pn, tint, tptr tvoid ]
   PROP ( writable_share sh;
        and (Z.le (Int.min_signed) x) (Z.le x (Int.max_signed));
        is_pointer_or_null v)
   PARAMS (b; Vint (Int.repr x); v) GLOBALS (gv)
-  SEP  (mem_mgr gv; node_lock_inv (Share.split gsh1).1 g n g_root lock;
+  SEP  (mem_mgr gv; node_lock_inv' (Share.split gsh1).1 g n g_root lock;
        pn_rep_1 g g_root Ews b n) | (tree_rep g g_root M)
   POST[ tint ]
-  EX pt : bool * ( val * (val * (val * (share * (gname * node_info)) )))%type,
+  EX pt : bool * (val * (val * (lock_handle * (share * (gname * node_info)))))%type,
   PROP ()
        (* (false, (p1, (pt, ( lock_in, (gsh, (g_in, r)))))) *)
        LOCAL (temp ret_temp (Val.of_bool pt.1))
@@ -155,7 +147,7 @@ Program Definition traverse_spec :=
                then ((pt.2.2.2.2.2.2).2 = Some None /\ pt.2.2.1 = nullval)
                else (pt.2.2.1 <> nullval /\
                (exists (v1: val) (g1 g2: gname),
-                   (pt.2.2.2.2.2.2).2 = Some (Some(x, v1, g1, g2)))))) && emp;
+                   (pt.2.2.2.2.2.2).2 = Some (Some(x, v1, g1, g2)))))) && seplog.emp;
              (node_lock_inv_new (pt.2.2.2.2.1) g (pt.2.1)
                                              (pt.2.2.2.2.2.1)
                                              (pt.2.2.2.1)
@@ -166,44 +158,39 @@ Program Definition traverse_spec :=
              )
        | (tree_rep g g_root M).
 
-
-Program Definition insertOp_spec :=
+Definition insertOp_spec :=
   DECLARE _insertOp
-          ATOMIC TYPE (rmaps.ConstType (bool * val * val * val * share * gname * node_info *
-                                       val *  share  * Z *  val * globals * gname * gname))
-          OBJ M INVS base.empty base.top
-   WITH fl, p, pt, lock_in, gsh, g_in, r, b, sh, x, v, gv, g , g_root
+  WITH b: val, sh: share, x: Z, v: val,
+              p : val, tp: val,
+              gv: globals
   PRE [ tptr t_struct_pn, tint, tptr tvoid ]
-  PROP ( readable_share sh; and (Z.le (Int.min_signed) x) (Z.le x (Int.max_signed));
+  PROP ( writable_share sh;
+       and (Z.le (Int.min_signed) x) (Z.le x (Int.max_signed));
          is_pointer_or_null v )
           PARAMS (b; Vint (Int.repr x); v) GLOBALS (gv)
           SEP  (mem_mgr gv;
-                 !!(fl = true /\ key_in_range x r.1 = true ∧
-                    r.2 = Some None /\ pt = nullval) && emp;
-                    (node_lock_inv_new gsh g p g_in lock_in pt r *
-                     data_at Ews t_struct_pn (p, p) b *
-                     my_half g_root (Share.split gsh1).2 (Neg_Infinity, Pos_Infinity, None)))
-                | (tree_rep g g_root M)
+                data_at sh (t_struct_pn) (p, p) b;
+                field_at Ews t_struct_tree_t (DOT _t) tp p)
   POST[ tvoid ]
-  PROP ()
+  EX (pnt p1' p2' : val) (lock1 lock2 : val),
+  PROP (pnt <> nullval)
         LOCAL ()
         SEP (mem_mgr gv;
-             EX pt : bool * (val * (val * (val * (share * (gname * node_info)))))%type,
-                 !!( pt.1 = true /\ pt.2.2.1 <> nullval) &&
-                   emp * (node_lock_inv_new (pt.2.2.2.2.1) g (pt.2.1)
-                                             (pt.2.2.2.2.2.1)
-                                             (pt.2.2.2.1)
-                                             (pt.2.2.1)
-                                             (pt.2.2.2.2.2.2)   *
-                        data_at Ews t_struct_pn (pt.2.1, pt.2.1) b *
-                        my_half g_root (Share.split gsh1).2 (Neg_Infinity, Pos_Infinity, None)))
-            | (tree_rep g g_root (<[x:=v]>M)).
-
+             data_at sh t_struct_pn (p, p) b;
+             field_at Ews t_struct_tree_t (DOT _t) pnt p;
+             malloc_token Ews t_struct_tree pnt;
+             malloc_token Ews t_struct_tree_t p1';
+             malloc_token Ews t_struct_tree_t p2';
+             atomic_int_at Ews (vint 0) lock1;
+             atomic_int_at Ews (vint 0) lock2;
+             data_at Ews t_struct_tree (vint x, (v, (p1', p2'))) pnt;
+             data_at Ews t_struct_tree_t (Vlong (Int64.repr (Int.signed (Int.repr 0))), lock1) p1';
+             data_at Ews t_struct_tree_t (Vlong (Int64.repr (Int.signed (Int.repr 0))), lock2) p2').
 
 Program Definition insert_spec :=
   DECLARE _insert2
-  ATOMIC TYPE (rmaps.ConstType (val *  share * val * Z * val * globals * gname * gname))
-  OBJ M INVS base.empty base.top
+  ATOMIC TYPE (rmaps.ConstType (val *  share * lock_handle * Z * val * globals * gname * gname))
+  OBJ M INVS ∅
   WITH  b, sh, lock, x, v, gv, g, g_root
   PRE [ tptr (tptr t_struct_tree_t), tint, tptr tvoid ]
           PROP (writable_share sh; and (Z.le Int.min_signed x)(Z.le x Int.max_signed);
@@ -215,16 +202,11 @@ Program Definition insert_spec :=
         LOCAL ()
        SEP (mem_mgr gv; nodebox_rep g g_root sh lock b) | (tree_rep g g_root (<[x:=v]>M)).
 
-Definition acquire_spec := DECLARE _acquire acquire_spec.
-Definition release2_spec := DECLARE _release2 release2_spec.
-Definition makelock_spec := DECLARE _makelock (makelock_spec _).
-Definition freelock2_spec := DECLARE _freelock2 (freelock2_spec _).
 Definition spawn_spec := DECLARE _spawn spawn_spec.
 
-
 Definition Gprog : funspecs :=
-    ltac:(with_library prog [acquire_spec; release2_spec; makelock_spec;
-    freelock2_spec; surely_malloc_spec; insert_spec; insertOp_spec; traverse_spec; findnext_spec;
+    ltac:(with_library prog [acquire_spec; release_spec; makelock_spec; free_atomic_spec;
+     surely_malloc_spec; traverse_spec; insertOp_spec; insert_spec; findnext_spec;
                             spawn_spec ]).
 
 Lemma node_rep_saturate_local:
@@ -234,7 +216,6 @@ Proof.
   rewrite node_rep_def. Intros tp. entailer!.
 Qed.
 Global Hint Resolve node_rep_saturate_local: saturate_local.
-
 Lemma node_rep_valid_pointer:
   forall t g g_current p, node_rep p g g_current t |-- valid_pointer p.
 Proof.
@@ -246,7 +227,8 @@ Global Hint Resolve node_rep_valid_pointer : valid_pointer.
 Lemma tree_rep_R_saturate_local:
    forall t p g_children g, tree_rep_R p t g_children g |-- !! is_pointer_or_null p.
 Proof.
-intros. unfold tree_rep_R. destruct (eq_dec p nullval). entailer!.
+intros. unfold tree_rep_R. change emp with seplog.emp.
+destruct (eq_dec p nullval). entailer !.
 Intros ga gb x v pa pb locka lockb. entailer!.
 Qed.
 Global Hint Resolve tree_rep_R_saturate_local: saturate_local.
@@ -254,11 +236,11 @@ Global Hint Resolve tree_rep_R_saturate_local: saturate_local.
 Lemma tree_rep_R_valid_pointer:
   forall t tp g_children g, tree_rep_R tp t g_children g |-- valid_pointer tp.
 Proof.
-intros. unfold tree_rep_R. destruct (eq_dec tp nullval). entailer!.
-Intros ga gb x v pa pb locka lockb. entailer!.
+  intros. unfold tree_rep_R. change emp with seplog.emp.
+  destruct (eq_dec tp nullval). entailer!.
+  Intros ga gb x v pa pb locka lockb. entailer!.
 Qed.
 Global Hint Resolve tree_rep_R_valid_pointer : valid_pointer.
-
 Lemma ltree_saturate_local:
   forall g g_root lsh gsh p lock, ltree g g_root lsh gsh p lock |-- !! isptr p.
 Proof.
@@ -296,35 +278,34 @@ Proof.
     entailer !.
 Qed.
 
-(* invariants for traverse *)
 Definition traverse_inv (b : val) (lock: val)
              (sh: share) (x: Z) (v: val) (g_root: gname)
-             gv (inv_names : invG) (g : gname) AS : environ -> mpred :=
-  (EX (r : node_info) (pnN : val) (gN_in : gname) (lockN_in : val) (gsh : share),
+             gv (inv_names : invariants.invG) (g : gname) AS : environ -> mpred :=
+  (EX (r : node_info) (pnN : val) (gN_in : gname) (lockN_in : lock_handle) (gsh : share),
             PROP (key_in_range x (fst r) = true)
                  LOCAL (temp _flag (vint 1); temp _pn__2 b;
                        temp _x (vint x); temp _value v; gvars gv)
                  SEP (pn_rep_1 g g_root sh b pnN;
                      (*pn->n*)
                      node_rep pnN g gN_in r;
-                     field_at lsh2 t_struct_tree_t [StructField _lock] lockN_in pnN;
-                     my_half gN_in gsh r; malloc_token Ews tlock lockN_in;
+                     field_at lsh2 t_struct_tree_t [StructField _lock] (ptr_of lockN_in) pnN;
+                     my_half gN_in gsh r;
                      |> lock_inv lsh2 lockN_in (node_lock_inv gsh g pnN gN_in lockN_in);
                      AS; mem_mgr gv))%assert.
 
 Definition traverse_inv_1 (b: val) (p: val) (g: gname) (g_root: gname) (g_in: gname)
-                          (lock_in: val) (gsh: share) (sh: share) (r: node_info) (x: Z) :=
+                          (lock_in: lock_handle) (gsh: share) (sh: share) (r: node_info) (x: Z) :=
   data_at sh (t_struct_pn) (p, p) b *
   my_half g_root (snd (Share.split gsh1)) (Neg_Infinity, Pos_Infinity, None) *
   field_at Ews t_struct_tree_t (DOT _t) nullval p *
   malloc_token Ews t_struct_tree_t p * in_tree g g_in *
-  field_at lsh2 t_struct_tree_t (DOT _lock) lock_in p *
+  field_at lsh2 t_struct_tree_t (DOT _lock) (ptr_of lock_in) p *
   my_half g_in gsh r * (!!(key_in_range x r.1 = true /\ r.2 = Some None) && emp) *
-  malloc_token Ews tlock lock_in * lock_inv lsh2 lock_in (node_lock_inv gsh g p g_in lock_in).
+  lock_inv lsh2 lock_in (node_lock_inv gsh g p g_in lock_in).
 
 Definition traverse_inv_2 (b: val) (p: val) (tp: val) (g: gname) (g_root: gname) (g_in: gname)
-                          (lock_in: val) (gsh: share) (sh: share) (r: node_info) (x: Z):=
-  EX (v1: val) (pa: val) (pb: val) (ga: gname) (gb: gname) (locka: val) (lockb: val),
+                          (lock_in: lock_handle) (gsh: share) (sh: share) (r: node_info) (x: Z):=
+  EX (v1: val) (pa: val) (pb: val) (ga: gname) (gb: gname) (locka lockb: lock_handle),
   data_at sh (t_struct_pn) (p, p) b *
   field_at Ews t_struct_tree_t (DOT _t) tp p *
   data_at Ews t_struct_tree (vint x, (v1, (pa, pb))) tp *
@@ -332,12 +313,11 @@ Definition traverse_inv_2 (b: val) (p: val) (tp: val) (g: gname) (g_root: gname)
   malloc_token Ews t_struct_tree_t p *
   in_tree g g_in * malloc_token Ews t_struct_tree tp *
   ltree g ga lsh1 gsh1 pa locka * ltree g gb lsh1 gsh1 pb lockb *
-  field_at lsh2 t_struct_tree_t (DOT _lock) lock_in p *
+  field_at lsh2 t_struct_tree_t (DOT _lock) (ptr_of lock_in) p *
   my_half g_in gsh r *
     (!!(key_in_range x r.1 = true ∧ r.2 = Some (Some (x, v1, ga, gb)) ∧
         (Int.min_signed ≤ x ≤ Int.max_signed)%Z /\
           is_pointer_or_null pa /\ is_pointer_or_null pb /\ is_pointer_or_null v1) && emp) *
-  malloc_token Ews tlock lock_in *
   lock_inv lsh2 lock_in (node_lock_inv gsh g p g_in lock_in).
 
 (*Proving traverse spec *)
@@ -348,9 +328,10 @@ Proof.
   Intros p.
   forward.
   set (AS := atomic_shift _ _ _ _ _ ).
-  forward_loop (traverse_inv b lock Ews x v g_root gv inv_names g AS)
+  forward_loop (traverse_inv b (ptr_of lock) Ews x v g_root gv inv_names g AS)
                break:
-    (EX (flag : bool) (q: val) (pt: val) (gsh: share) (g_in: gname) (lock_in : val) (r : node_info),
+    (EX (flag : bool) (q: val) (pt: val) (gsh: share) (g_in: gname)
+       (lock_in : lock_handle) (r : node_info),
                 PROP() LOCAL(temp _flag (Val.of_bool flag))
                       SEP((if flag
                           then ((traverse_inv_1 b q g g_root g_in lock_in gsh Ews r x) *
@@ -359,9 +340,8 @@ Proof.
                                   (!!(pt <> nullval) && emp))) *
                            Q (flag, (q, (pt, (lock_in, (gsh, (g_in, r)))))) * mem_mgr gv)).
   - (*pre-condition*)
-    unfold traverse_inv.
+    unfold traverse_inv, node_lock_inv'.
     unfold node_lock_inv at 1.
-    rewrite selflock_eq.
     unfold node_lock_inv_pred at 1.
     unfold sync_inv.
     Intro r.
@@ -396,6 +376,7 @@ Proof.
     assert_PROP(is_pointer_or_null tp) by entailer !.
     unfold tree_rep_R.
     forward.
+    change emp with seplog.emp.
     (* if *)
     forward_if.
     + (* if (pn->p->t == NULL) *)
@@ -403,10 +384,10 @@ Proof.
       entailer !.
       Intros ga gb x0 v1 pa pb locka lockb.
       entailer !.
-    + rewrite H3.
-      (*  Q (true, (p1, (p1, (lock_in, (gsh, g_in))))) *)
+    + rewrite H3. (*  Q (true, (p1, (p1, (lock_in, (gsh, g_in))))) *)
       gather_SEP AS (my_half g_in _ _) (in_tree g _).
-      viewshift_SEP 0 (EX y, Q y * (!!( y = (true, (pn, (nullval, (lock_in, (gsh, (g_in, r)))))))
+      viewshift_SEP 0 (EX y, Q y *
+                               (!!( y = (true, (pn, (nullval, (lock_in, (gsh, (g_in, r)))))))
                                     && (in_tree g g_in * my_half g_in gsh r))).
       {
         go_lower.
@@ -493,61 +474,80 @@ Proof.
         }
         (* b != 0 *)
         destruct succ as (succ & n').
-        simpl in *.
         destruct succ.
         destruct H8 as [Hpa | Hpb].
         * unfold ltree.
           destruct Hpa as (Hpa & Hx).
+          simpl in Hpa.
+          simpl.
           Intros.
           forward.
           subst n'.
           forward.
           (*acquire*)
-          forward_call (locka, lsh1, node_lock_inv gsh1 g pa ga locka).
-          unfold node_lock_inv at 2.
-          rewrite selflock_eq.
-          unfold node_lock_inv_pred at 1.
-          unfold sync_inv at 1.
+          forward_call acquire_inv_simple (lsh1, locka, node_lock_inv gsh1 g pa ga locka).
+          Intros.
+          forward.
+          gather_SEP (lock_inv lsh1 locka (node_lock_inv gsh1 g pa ga locka))
+            (node_lock_inv gsh1 g pa ga locka).
+          unfold node_lock_inv at 1.
+          unfold node_lock_inv at 1.
+          sep_apply self_part_eq.
+          assert (lsh2 <> Share.bot).
+          { apply readable_not_bot. apply readable_lsh2. }
+          auto.
+          unfold node_lock_inv_pred at 3.
+          unfold sync_inv.
           Intros a.
           rewrite node_rep_def.
           Intros tp1.
           forward.
-          forward.
           gather_SEP AS (my_half g_in _ _) (in_tree g g_in) (my_half ga gsh1 a); unfold AS.
-          sep_apply (
-              in_tree_left_range (bool * (val * (val * (val * (share * (gname *
+          viewshift_SEP 0 (atomic_shift (λ M, tree_rep g g_root M) ⊤ ∅
+                             (λ (M : gmap key val) (_ : bool *
+                                       (val * (val * (lock_handle * (share * (gname * node_info)))))),
+               fold_right_sepcon [tree_rep g g_root M]) 
+                             Q * my_half g_in gsh r *
+                             (EX ba, !! (less_than_equal ba r.1.1 = true /\
+                range_incl a.1 (ba, Finite_Integer x0) = true) &&
+            (in_tree g g_in * my_half ga gsh1 (ba, Finite_Integer x0, a.2)))).
+          {
+            go_lower.
+            apply (in_tree_left_range (bool * (val * (val * (val * namespace * gname * (share * (gname *
                                  (range * option (option ghost_info))))))))
-            (λ M (_ : (bool * (val * (val * (val * (share * (gname *
+            (λ M (_ : (bool * (val * (val * (val * namespace * gname * (share * (gname *
                                  (range * option (option ghost_info))))))))),
-              tree_rep g g_root M * emp) Q x x0 g g_root inv_names v1 g_in ga gb).
-          rewrite ! Int.signed_repr in Hx; by rep_lia.
+              fold_right_sepcon [tree_rep g g_root M]) Q x x0 g g_root v1 g_in ga gb).
+            auto. auto. rewrite ! Int.signed_repr in Hx; by rep_lia.
+          }
           Intros ba.
           (*release*)
-          forward_call (lock_in, lsh2,
-                        node_lock_inv_pred gsh g pn g_in lock_in,
-                        node_lock_inv gsh g pn g_in lock_in).
+          forward_call release_self (lsh2, lock_in,
+                    node_lock_inv_pred gsh g pn g_in (ptr_of lock_in)).
           {
-            lock_props.
-            unfold node_lock_inv at 4.
-            fold (node_lock_inv gsh1 g pa ga locka).
-            rewrite selflock_eq.
-            unfold node_lock_inv_pred at 1.
-            unfold sync_inv at 1.
+            unfold node_lock_inv.
+            cancel.
+            unfold node_lock_inv_pred at 4.
+            unfold sync_inv.
             Exists r.
             rewrite node_rep_def.
-            Exists tp; cancel.
-            unfold tree_rep_R at 2.
-            rewrite -> if_false by auto.
-            Exists ga gb x0 v1 pa pb locka lockb.
-            unfold ltree at 1; entailer !.
-            repeat rewrite later_sepcon.
-            entailer !.
-            unfold node_lock_inv at 3.
-            unfold ltree.
-            entailer !.
-            repeat rewrite later_sepcon.
+            Exists tp.
             cancel.
+            unfold tree_rep_R at 2.
+            rewrite -> if_false; auto.
+            Exists ga gb x0 v1 pa pb locka lockb.
+            unfold ltree at 1. entailer !.
+            repeat rewrite later_sepcon.
+            entailer !.
+            unfold node_lock_inv.
+            cancel.
+            unfold ltree.
+            unfold node_lock_inv.
+            entailer !.
+            repeat rewrite later_sepcon.
+            entailer !.
           }
+          (* proving |--  traverse_inv b (ptr_of lock) Ews x v g_root gv inv_names g AS *)
           unfold traverse_inv.
           Exists (ba, Finite_Integer x0, a.2) pa ga locka gsh1.
           unfold node_lock_inv.
@@ -568,57 +568,81 @@ Proof.
           Exists pn.
           entailer !.
           apply range_incl_tree_rep_R; auto.
-        * unfold ltree.
-          destruct Hpb as (Hpb & Hx).
-          Intros.
-          forward.
-          subst n'.
-          forward.
-          (*acquire*)
-          forward_call (lockb, lsh1, node_lock_inv gsh1 g pb gb lockb).
-          unfold node_lock_inv at 2.
-          rewrite selflock_eq.
-          unfold node_lock_inv_pred at 1.
-          unfold sync_inv at 1.
-          Intros a.
-          rewrite node_rep_def.
-          Intros tp1.
-          forward.
-          forward.
-          gather_SEP AS (my_half g_in _ _) (in_tree g g_in) (my_half gb gsh1 a); unfold AS.
-          sep_apply (in_tree_right_range (bool * (val * (val * (val * (share * (gname *
-                                         (range * option (option ghost_info))))))))
-            (λ M (_ : (bool * (val * (val * (val * (share * (gname *
-                                         (range * option (option ghost_info))))))))),
-              tree_rep g g_root M * emp) Q x x0 g g_root inv_names v1 g_in ga gb).
-          rewrite ! Int.signed_repr in Hx; by rep_lia.
+       * unfold ltree.
+         destruct Hpb as (Hpb & Hx).
+         simpl in Hpb.
+         simpl.
+         Intros.
+         forward.
+         subst n'.
+         forward.
+         (*acquire*)
+         forward_call acquire_inv_simple (lsh1, lockb, node_lock_inv gsh1 g pb gb lockb).
+         Intros.
+         forward. 
+         gather_SEP (lock_inv lsh1 lockb (node_lock_inv gsh1 g pb gb lockb))
+            (node_lock_inv gsh1 g pb gb lockb).
+         unfold node_lock_inv at 1.
+         unfold node_lock_inv at 1.
+         sep_apply self_part_eq.
+         assert (lsh2 <> Share.bot). 
+         { apply readable_not_bot. 
+           apply readable_lsh2.
+         }
+         auto.
+         unfold node_lock_inv_pred at 3.
+         unfold sync_inv.
+         Intros a.
+         rewrite node_rep_def.
+         Intros tp1.
+         forward.
+         gather_SEP AS (my_half g_in _ _) (in_tree g g_in) (my_half gb gsh1 a); unfold AS.
+         viewshift_SEP 0 (
+             atomic_shift (λ M : gmap key val, tree_rep g g_root M) ⊤ ∅ (λ (M : gmap key val) (_ : bool *
+                                       (val * (val * (lock_handle * (share * (gname * node_info)))))),
+               fold_right_sepcon [tree_rep g g_root M])  Q *
+                      my_half g_in gsh r *
+                      (EX ta : number,
+                       !! (less_than_equal r.1.2 ta = true
+                           ∧ range_incl a.1 (Finite_Integer x0, ta) = true) &&
+                       (in_tree g g_in * my_half gb gsh1 (Finite_Integer x0, ta, a.2)))).
+         {
+           go_lower.
+           apply (in_tree_right_range (bool * (val * (val * (val * namespace * gname * (share * (gname *
+                                 (range * option (option ghost_info))))))))
+            (λ M (_ : (bool * (val * (val * (val * namespace * gname * (share * (gname *
+                                 (range * option (option ghost_info))))))))),
+              fold_right_sepcon [tree_rep g g_root M]) Q x x0 g g_root v1 g_in ga gb).
+            auto. auto. rewrite ! Int.signed_repr in Hx; by rep_lia.
+          }
           Intros ba.
           (*release*)
-          forward_call (lock_in, lsh2,
-                        node_lock_inv_pred gsh g pn g_in lock_in,
-                        node_lock_inv gsh g pn g_in lock_in).
+          forward_call release_self (lsh2, lock_in,
+                    node_lock_inv_pred gsh g pn g_in (ptr_of lock_in)).
           {
-            lock_props.
-            unfold node_lock_inv at 4.
-            fold (node_lock_inv gsh1 g pb gb lockb).
-            rewrite selflock_eq.
-            unfold node_lock_inv_pred at 1.
-            unfold sync_inv at 1.
+            unfold node_lock_inv.
+            cancel.
+            unfold node_lock_inv_pred at 4.
+            unfold sync_inv.
             Exists r.
             rewrite node_rep_def.
-            Exists tp; cancel.
-            unfold tree_rep_R at 2.
-            rewrite -> if_false by auto.
-            Exists ga gb x0 v1 pa pb locka lockb.
-            unfold ltree at 1; entailer !.
-            repeat rewrite later_sepcon.
-            entailer !.
-            unfold node_lock_inv at 3.
-            unfold ltree.
-            entailer !.
-            repeat rewrite later_sepcon.
+            Exists tp.
             cancel.
+            unfold tree_rep_R at 2.
+            rewrite -> if_false; auto.
+            Exists ga gb x0 v1 pa pb locka lockb.
+            unfold ltree at 1. entailer !.
+            repeat rewrite later_sepcon.
+            entailer !.
+            unfold node_lock_inv.
+            cancel.
+            unfold ltree.
+            unfold node_lock_inv.
+            entailer !.
+            repeat rewrite later_sepcon.
+            entailer !.
           }
+          (* proving |--  traverse_inv b (ptr_of lock) Ews x v g_root gv inv_names g AS *)
           unfold  traverse_inv.
           Exists (Finite_Integer x0, ba, a.2) pb gb lockb gsh1.
           unfold node_lock_inv.
@@ -641,27 +665,28 @@ Proof.
           apply range_incl_tree_rep_R; auto.
         * (* b == 0*)
           apply repr_inj_unsigned' in H9; rep_lia.
-      }
+    }
   - (* semax Delta (PROP ( )  RETURN ( ) SEP ()) (return _flag;) POSTCONDITION *)
     Intros flag.
     Intros p1 pt gsh g_in lock_in r.
     forward.
-    unfold traverse_inv_1, traverse_inv_2; unfold node_lock_inv_new.
+    unfold traverse_inv_1, traverse_inv_2, node_lock_inv_new.
     destruct flag.
     Intros. (* will have key_in_range x r.1 = true for post condition*)
-
     + (* flag = 1 *)
       Intros.
       Exists (true, (p1, (nullval, (lock_in, (gsh , (g_in, r)))))).
       simpl in *.
       unfold tree_rep_R.
       erewrite eq_dec_refl. (* will have key_in_range x r.1 = true *)
+      change emp with seplog.emp.
       entailer !.
     + (* flag = 0*)
       Intros v1 pa pb ga gb locka lockb.
       Intros.
       Exists (false, (p1, (pt, (lock_in, (gsh, (g_in, r)))))).
       simpl in *.
+      change emp with seplog.emp.
       entailer !.
       exists v1, ga, gb; auto.
       unfold tree_rep_R.
@@ -671,160 +696,60 @@ Proof.
         unfold node_lock_inv; entailer !.
 Qed.
 
-
-(* proving insertOp function *)
 Lemma insertOp: semax_body Vprog Gprog f_insertOp insertOp_spec.
 Proof.
+  Check node_lock_inv.
   start_function.
-  set (AS := atomic_shift _ _ _ _ _).
+  change emp with seplog.emp.
   Intros.
-  simpl.
-  unfold node_lock_inv_new.
-  subst pt.
-  unfold tree_rep_R.
-  destruct (eq_dec nullval nullval); last contradiction.
+   (* (false, (p1, (pt, ( lock_in, (gsh, (g_in, r)))))) *)
   Intros.
   forward_call (t_struct_tree_t, gv).
   Intros p1'.
   forward_call (t_struct_tree_t, gv).
   Intros p2'.
   forward.
+  (* unfold_data_at (data_at _ _ _ p1'). *)
   assert_PROP (field_compatible t_struct_tree_t [] p1') by entailer!.
-  simpl.
   forward. (* p1->t=NULL *)
+  (* unfold_data_at (data_at _ _ _ p2'). *)
   assert_PROP (field_compatible t_struct_tree_t [] p2') by entailer!.
-  simpl.
-  forward_call (tlock, gv).
-  { simpl. rewrite Z.max_r. repeat (split; auto); rep_lia. rep_lia. }
-  Intros l1.
-  unfold tlock.
-  destruct r as [p1 o].
-  destruct p1.
-  simpl in H3; subst.
-  gather_SEP AS (my_half g_in _  _)  (in_tree g  _).
-  viewshift_SEP 0
-    ( Q
-      * (EX g1 g2:gname, EX n1 n2:number,
-           (!!(key_in_range x (n1,n2) = true) &&
-              my_half g_in gsh (n1, n2, Some (Some(x,v,g1,g2))) *
-              in_tree g g_in *
-              my_half g1 gsh1 (n1, Finite_Integer x, Some (@None ghost_info)) *
-              my_half g2 gsh1 (Finite_Integer x, n2, Some (@None ghost_info)) *
-              in_tree g g1 * in_tree g g2))).
-  {
-    go_lower.
-    eapply sync_commit_gen1.
-    intros.
-    iIntros "[H1 H2]".
-    iModIntro.
-    iPoseProof (tree_rep_insert with "[$H1 $H2]") as "Hadd".
-    iDestruct "Hadd" as (r o0) "([Hmy H1] & H2)".
-    iExists (r, Some o0). iFrame. iDestruct "H2" as "[[Hnew _] _]".
-    iIntros "H"; iDestruct "H" as %Hsub.
-    iMod "Hnew".
-    iDestruct "Hnew" as (g1 g2) "H".
-    iModIntro.
-    iExists (r, Some (Some(x, v, g1, g2))).
-    iExists (r, Some (Some (x, v, g1, g2))).
-    apply node_info_incl' in Hsub as [? Heq]. simpl snd in *. inv Heq.
-    logic_to_iris. iSplit.
-    {
-      iPureIntro.
-      intros ? Hincl.
-      destruct b0 as ((n3, n4), i).
-      hnf.
-      simpl.
-      destruct (range_incl_join _ _ _ Hincl).
-      simpl in *; subst. split; [|reflexivity].
-      split.
-      { symmetry; rewrite merge_comm; apply merge_range_incl'; auto. }
-      destruct Hincl as [_ Hincl]; simpl in Hincl.
-      inv Hincl; try constructor.
-      inv H10.
-    }
-    iIntros "(H1 & H2)".
-    instantiate (1 := x).
-    instantiate (1:= v).
-    iSpecialize ("H" with "[$H2 $Hmy]").
-    iSplit; auto.
-    {
-      iPureIntro.
-      split; auto.
-      eapply key_in_range_incl; eassumption. }
-      iDestruct "H" as "(((((? & ?) & ?) & ?) & ?) & ?)".
-      iModIntro. rewrite exp_sepcon1; iExists tt.
-      rewrite !exp_sepcon2; iExists g1.
-      rewrite !exp_sepcon2; iExists g2.
-      rewrite !exp_sepcon2; iExists r.1.
-      rewrite !exp_sepcon2; iExists r.2; destruct r; iFrame.
-      iPureIntro; split; auto.
-      eapply key_in_range_incl; eassumption.
-    }
-    Intros g1 g2 n1 n2.
-    Typeclasses eauto:= 2.
-    forward_call (l1, Ews, node_lock_inv gsh1 g p1' g1 l1).
-    forward. (*p1->lock = l1*)
-    rewrite <- (lock_inv_share_join lsh1 lsh2) by auto.
-    Typeclasses eauto:= 6.
-    forward_call (l1, lsh2, node_lock_inv_pred gsh1 g p1' g1 l1, node_lock_inv gsh1 g p1' g1 l1).
-    { lock_props.
-      unfold node_lock_inv at 4.
-      rewrite selflock_eq .
-      unfold node_lock_inv_pred at 1.
-      unfold sync_inv at 1.
-      Exists (n1, Finite_Integer x, Some (@None ghost_info)).
-      rewrite node_rep_def.
-      Exists nullval.
-      unfold_data_at (data_at _ _ _ p1').
-      erewrite <- (field_at_share_join _ _ _ _ [StructField _lock]) by eauto.
-      unfold tree_rep_R.
-      simpl.
-      unfold node_lock_inv at 2. entailer!.
-    }
-    forward_call (tlock, gv).
-    { simpl.  rewrite Z.max_r. repeat (split; auto); rep_lia. rep_lia. }
-    Intros l2.
-    forward_call (l2, Ews, (node_lock_inv gsh1 g p2' g2 l2)).
-    forward. (*p2->lock = l2*)
-    rewrite <- (lock_inv_share_join lsh1 lsh2) by auto.
-    forward_call (l2, lsh2, node_lock_inv_pred gsh1 g p2' g2 l2, node_lock_inv gsh1 g p2' g2 l2).
-    { lock_props.
-      unfold node_lock_inv at 5.
-      rewrite selflock_eq .
-      unfold node_lock_inv_pred at 1.
-      unfold sync_inv at 1.
-      Exists (Finite_Integer x,n2,Some (@None ghost_info)).
-      rewrite node_rep_def.
-      Exists nullval.
-      unfold_data_at (data_at _ _ _ p2').
-      erewrite <- (field_at_share_join _ _ _ _ [StructField _lock]) by eauto.
-      unfold tree_rep_R. simpl. unfold node_lock_inv at 2. entailer!.
-    }
-    forward_call (t_struct_tree, gv).
-    Intros p'.
-    repeat forward.
-    unfold node_lock_inv_new.
-    (* (false, (p1, (pt, ( lock_in, (gsh, (g_in, r)))))) *)
-    Exists (true, (p, (p', (lock_in, (gsh, (g_in, (n1, n2, Some (Some (x, v, g1, g2))) )))))) .
-    entailer !.
-    unfold tree_rep_R.
-    assert_PROP (p' <> nullval) by entailer!.
-    rewrite -> if_false.
-    Exists g1 g2 x v p1' p2' l1 l2.
-    unfold ltree.
-    entailer !.
-    rewrite <- later_sepcon.
-    setoid_rewrite sepcon_comm at 1.
-    setoid_rewrite sepcon_comm at 3.
-    setoid_rewrite sepcon_comm at 6.
-    rewrite <- sepcon_assoc.
-    rewrite <- sepcon_assoc.
-    rewrite <- sepcon_assoc.
-    apply now_later.
-    auto.
+  forward_call (gv).
+  Intros lock1.
+  forward.
+  sep_apply atomic_int_isptr.
+  Intros.
+  forward_call release_nonatomic (lock1).
+  forward_call (gv).
+  Intros lock2.
+  forward.
+  Intros.
+  forward_call release_nonatomic (lock2).
+  (* make lock invariant *)
+  forward_call (t_struct_tree, gv).
+  Intros pnt.
+  forward. forward. forward. forward. forward. forward. forward.
+  forward. forward. forward. forward. forward. forward. forward.
+  Exists pnt p1' p2' lock1 lock2.
+  entailer !.
 Qed.
 
-(* proving insert function *)
+Lemma make_lock_inv_0_self : forall v N R sh1 sh2, sh1 <> Share.bot -> sepalg.join sh1 sh2 Ews ->
+    (atomic_int_at Ews (vint 0) v * R) |-- @fupd mpred (bi_fupd_fupd(BiFUpd := mpred_bi_fupd)) ⊤ ⊤ (EX h, !!(ptr_of h = v /\ name_of h = N) && lock_inv sh1 h (R * self_part sh2 h)).
+Proof.
+  intros.
+  iIntros "[a R]".
+  iDestruct (atomic_int_isptr with "a") as %Ha.
+  iMod (own_alloc(RA := VST.concurrency.cancelable_invariants.share_ghost) with "[$]")
+      as (g) "g"; first done.
+  setoid_rewrite (own_op(RA := VST.concurrency.cancelable_invariants.share_ghost) _ _ _ _ _ H0);
+    iDestruct "g" as "[g1 g2]".
+  iMod (inv_alloc with "[a R g2]") as "I";
+      [| iExists (v, N, g); unfold lock_inv; simpl; iFrame; auto].
+  iIntros "!>"; unfold inv_for_lock.
+  iLeft; iExists false; iFrame; auto.
+Qed.
+
 Lemma body_insert: semax_body Vprog Gprog f_insert2 insert_spec.
 Proof.
   start_function.
@@ -838,276 +763,456 @@ Proof.
   forward.
   set (AS := atomic_shift _ _ _ _ _).
   (* acquire(pn->n->lock); *)
-  Check λ M : gmap key val, tree_rep g g_root M.
-  forward_call (lock, sh, (node_lock_inv (fst (Share.split gsh1)) g np g_root lock)).
-  set Q1:= fun (b : (bool * ( val * (val * (val * (share * (gname * node_info))))))%type) =>
-              if b.1
-              then AS
-              else AS.
-  (* traverse(pn, x, value) *)
-   forward_call (nb, np, sh,  lock, x, v, gv, g, g_root, Q1, inv_names).
-   {
-     unfold AS, pn_rep_1.
-     Exists Vundef.
-     entailer !.
-     rewrite !sepcon_assoc sepcon_comm.
-     rewrite !sepcon_assoc sepcon_comm.
-     rewrite ->  sepcon_assoc; apply sepcon_derives; [|cancel].
-     iIntros "AS".
-     unfold atomic_shift.
-     iAuIntro.
-     rewrite /atomic_acc /=.
-     iMod "AS" as (m) "Hm".
-     iDestruct "Hm" as "[H1 H2]".
-     iModIntro.
-     iExists m.
-     iFrame "H1".
-     iSplit; iFrame.
-     { iApply bi.and_elim_l; iFrame. }
-     {
-       iPoseProof (bi.and_elim_l with "H2") as "H2".
-       iIntros (pt) "[H H1]".
-       iMod ("H2" with "H") as "H".
-       iModIntro.
-       unfold Q1.
-       destruct (decide (pt.1 = true)).
-       { rewrite e; iFrame. }
-       { apply not_true_is_false in n; rewrite n; iFrame. }
-     }
-   }
-   Intros pt.
-   destruct pt as (fl & (p1 & (tp & (lock_in & (gsh & (g_in & (x0 & r))))))).
-   simpl in H2, H3.
-   destruct fl.
-   - destruct H3.
-     subst tp.
-     forward_if (PROP ( )
-                 LOCAL (temp _t'2 Vtrue; temp _t'8 lock; temp _t'7 np; temp _t'9 np;
+  forward_call acquire_inv_simple (sh, lock, node_lock_inv (Share.split gsh1).1 g np g_root lock).
+  {
+    set Q1:= fun (b : (bool * ( val * (val * (lock_handle * (share * (gname * node_info))))))%type) =>
+              if b.1 then AS else AS.
+    (* traverse(pn, x, value) *)
+    forward_call (nb, np, sh , lock, x, v, gv, g, g_root, Q1).
+    {
+      unfold pn_rep_1.
+      unfold node_lock_inv'.
+      Exists (default_val t_struct_pn).1.
+      unfold node_lock_inv.
+      sep_apply self_part_eq.
+      assert (lsh2 <> Share.bot).
+      { apply readable_not_bot. apply readable_lsh2. }
+      auto.
+      entailer !.
+      rewrite -> 2sepcon_assoc. rewrite sepcon_comm.
+      rewrite -> sepcon_assoc; apply sepcon_derives; [|cancel].
+      unfold atomic_shift; iIntros "AU"; iAuIntro; unfold atomic_acc; simpl.
+      iMod "AU" as (m) "[Hm HClose]".
+      iModIntro.
+      iExists m.
+      iFrame "Hm".
+      iSplit; iFrame.
+      { by iApply bi.and_elim_l. }
+      {
+        iDestruct "HClose" as "[HClose _]".
+        iIntros (pt) "[H _]".
+        iMod ("HClose" with "H") as "H".
+        iModIntro.
+        unfold Q1.
+        destruct (decide (pt.1 = true)). { rewrite e; iFrame. }
+        { apply not_true_is_false in n; rewrite n; iFrame. }
+      }
+    }
+    Intros pt.
+    destruct pt as (fl & (p1 & (tp & (lock_in & (gsh & (g_in & (x0 & r))))))).
+    simpl in H2, H3.
+    destruct fl.
+    simpl.
+    - destruct H3.
+      forward_if (PROP ( )
+                 LOCAL (temp _t'2 Vtrue; temp _t'8 (ptr_of lock); temp _t'7 np; temp _t'9 np;
                         temp _pn__2 nb; gvars gv; temp _t b; temp _x (vint x); temp _value v)
-                 SEP (Q; mem_mgr gv;
-                      EX pt : bool * (val * (val * (val * (share * (gname * node_info))))),
-                      !! (pt.1 = true  /\ pt.2.2.1 <> nullval) && emp *
+                 SEP (|={⊤}=> (|={⊤}=> Q * mem_mgr gv *
+                      EX pt : bool * (val * (val * (lock_handle * (share * (gname * node_info))))),
+                      !! (pt.1 = true  /\ pt.2.2.1 <> nullval) && seplog.emp *
                          (node_lock_inv_new pt.2.2.2.2.1 g pt.2.1
                            pt.2.2.2.2.2.1 pt.2.2.2.1 pt.2.2.1 pt.2.2.2.2.2.2 *
                          data_at Ews t_struct_pn (pt.2.1, pt.2.1) nb *
                          my_half g_root (Share.split gsh1).2 (Neg_Infinity, Pos_Infinity, None) *
                          data_at sh (tptr t_struct_tree_t) np b *
-                         field_at sh t_struct_tree_t (DOT _lock) lock np *
+                         field_at sh t_struct_tree_t (DOT _lock) (ptr_of lock) np *
                          lock_inv sh lock (node_lock_inv (Share.split gsh1).1 g np g_root lock) *
-                         malloc_token Ews t_struct_pn nb))).
-     + contradiction.
-     + (* insertOp(pn, x, value) *)
-       forward_call(true, p1, nullval, lock_in, gsh, g_in, (x0, r),
-                     nb, sh, x, v, gv, g , g_root, Q , inv_names).
-       {
-         Intros.
-         entailer !.
-         unfold Q1.
-         simpl.
-         unfold AS.
-         rewrite !sepcon_assoc.
-         apply sepcon_derives; [|cancel].
-         iIntros "AS".
-         unfold atomic_shift.
-         iAuIntro.
-         rewrite /atomic_acc /=.
-         iMod "AS" as (x1) "Hm".
-         iModIntro.
-         iDestruct "Hm" as "[H1 H2]".
-         iExists x1.
-         iFrame "H1".
-         iSplit.
-         { iApply bi.and_elim_l. iFrame. }
-         { iPoseProof (bi.and_elim_r with "H2") as "H2". iFrame. }
-      }
-      unfold Q1.
-      Intros pt.
-      destruct pt as (fl2 & (p2 & (tp2 & (lock_in2 & (gsh2 & (g_in2 & r2)))))).
-      entailer !.
-      Exists (fl2, (p2, (tp2, (lock_in2, (gsh2, (g_in2, r2)))))).
-      entailer !.
-      cancel.
-    + unfold node_lock_inv_new.
-      Intros pt.
-      destruct pt as (fl2 & (p2 & (tp2 & (lock_in2 & (gsh2 & (g_in2 & r2)))))).
-      simpl.
-      simpl in H4, H5.
-      forward.
-      forward.
-      (* _release2(_t'4) *)
-      unfold tree_rep_R.
-      rewrite if_false; auto.
-      Intros g1 g2 x1 v1 p1' p2' l1 l2.
-      (*  (_release2(_t'4); *)
-      forward_call (lock_in2, lsh2, node_lock_inv_pred gsh2 g p2 g_in2 lock_in2,
-                     node_lock_inv gsh2 g p2 g_in2 lock_in2).
-      {
-        lock_props.
-        unfold node_lock_inv at 3.
-        rewrite selflock_eq.
-        unfold node_lock_inv_pred at 1.
-        unfold sync_inv at 1.
-        destruct r2 as [p o].
-        simpl in H6, H9.
-        destruct p as [n1 n2].
-        Exists (n1, n2, Some (Some(x1, v1, g1, g2))).
-        rewrite node_rep_def.
-        unfold node_lock_inv.
-        Exists tp2; cancel.
-        unfold tree_rep_R. 
-        assert_PROP (tp2 <> nullval) by entailer!.
-        rewrite -> if_false by auto.
-        Exists g1 g2 x1 v1 p1' p2' l1 l2.
-        unfold ltree.
-        entailer !.
-        rewrite <- later_sepcon;
-          eapply derives_trans;
-          [|apply sepcon_derives, derives_refl; apply now_later].
-        entailer !.
-     }
-     gather_SEP Q (my_half _ _ _).
-     forward_call (t_struct_pn, nb, gv).
-     {
-       assert_PROP (nb <> nullval) by entailer !.
-       rewrite if_false; auto.
-       cancel.
-     }
-     unfold nodebox_rep.
-     entailer !.
-     Exists np.
-     unfold ltree, node_lock_inv.
-     entailer !.
-   - (* (_t'6->_value) = _value;) *)
-     forward_if (
-         PROP ( )
-           LOCAL (temp _t'2 Vfalse; temp _t'8 lock; temp _t'7 np; temp _t'9 np; temp _pn__2 nb;
-                  gvars gv; temp _t b; temp _x (vint x); temp _value v)
-           SEP (Q1 (false, (p1, (tp, (lock_in, (gsh, (g_in, (x0, r))))))); mem_mgr gv; emp;
-                field_at Ews t_struct_tree_t (DOT _t) tp p1 *
-                  malloc_token Ews t_struct_tree_t p1 * in_tree g g_in *
-                  (EX (ga gb : gname) (x1 : Z) (v0 pa pb locka lockb : val),
-                    !! ((x0, r).2 = Some (Some (x1, v0, ga, gb))
-                        ∧ (Int.min_signed ≤ x1 ≤ Int.max_signed)%Z
-                        ∧ is_pointer_or_null pa
-                        ∧ is_pointer_or_null pb ∧ tc_val (tptr Tvoid) v0 ∧
-                          key_in_range x1 (x0, r).1 = true) &&
-                      data_at Ews t_struct_tree (vint x1, (v, (pa, pb))) tp *
-                      malloc_token Ews t_struct_tree tp *
-                      |> ltree g ga lsh1 gsh1 pa locka *
-                      |> ltree g gb lsh1 gsh1 pb lockb) *
-                  my_half g_in gsh (x0, r) *
-                  field_at lsh2 t_struct_tree_t (DOT _lock) lock_in p1 *
-                  malloc_token Ews tlock lock_in *
-                  |> lock_inv lsh2 lock_in (node_lock_inv gsh g p1 g_in lock_in);
-                data_at Ews t_struct_pn (p1, p1) nb;
-                my_half g_root (Share.split gsh1).2 (Neg_Infinity, Pos_Infinity, None);
-                data_at sh (tptr t_struct_tree_t) np b;
-                field_at sh t_struct_tree_t (DOT _lock) lock np;
-                lock_inv sh lock (node_lock_inv (Share.split gsh1).1 g np g_root lock);
-                malloc_token Ews t_struct_pn nb)).
-     + destruct H3 as ( ?  & v2 & g21 & g22 & ?).
-       unfold node_lock_inv_new.
-       unfold tree_rep_R.
-       rewrite -> if_false by auto.
-       simpl in *.
-       Intros g1 g2 x1 v1 p1' p2' l1 l2.
-       forward.
-       forward.
-       forward.
-       Exists g1 g2 x1 v1 p1' p2' l1 l2.
-       entailer !.
-     + (* contradiction, since  Int.one = Int.zero *)
-       pose proof Int.one_not_zero; contradiction.
-     + unfold node_lock_inv_new, tree_rep_R.
-       destruct H3 as ( ? & v2 & g21 & g22 & ?).
-       Intros g1 g2 x1 v1 p1' p2' l1 l2.
-       forward.
-       forward.
-       simpl in H5. rewrite H5 in H4. injection H4.
-       intros. subst x1. subst v2. subst g21. subst g22.
-       unfold Q1.
-       simpl.
-       gather_SEP AS (my_half g_in _ _) (in_tree g  _).
-       viewshift_SEP 0 (Q *
-                  (EX n1 n2:number,
-                    !!(key_in_range x (n1,n2) = true) 
-                    && my_half g_in gsh (n1,n2,Some (Some(x,v,g1,g2))) * in_tree g g_in)).
+                         malloc_token Ews t_struct_pn nb)))); try contradiction.
+      + (* insertOp(pn, x, value) *)
+        unfold Q1.
+        Intros.
+        simpl.
+        change emp with seplog.emp.
+        forward_call(nb, Ews, x, v, p1, tp, gv).
+        { unfold node_lock_inv_new. rewrite H4; cancel. }
+        Intros pt.
+        destruct x0.
+        subst r.
+        gather_SEP AS (my_half g_in _  _)  (in_tree g  _).
+        replace_SEP 0 (
+            (|={⊤}=> Q * (EX g1 g2:gname, EX n1 n2:number,
+                              (!!(key_in_range x (n1,n2) = true) &&
+                                 my_half g_in gsh (n1, n2, Some (Some(x,v,g1,g2))) *
+                                 in_tree g g_in *
+                                 my_half g1 gsh1 (n1, Finite_Integer x, Some (@None ghost_info)) *
+                                 my_half g2 gsh1 (Finite_Integer x, n2, Some (@None ghost_info)) *
+                                 in_tree g g1 * in_tree g g2)))).
         {
           go_lower.
           eapply sync_commit_gen1.
-          intros. iIntros "H".
-          iDestruct "H" as "[H1 H2]".
+          intros.
+          iIntros "[H1 H2]".
           iModIntro.
-          iPoseProof (tree_rep_insert with "[$H1 $H2]") as "Hadd". 
-          iDestruct "Hadd" as ((n1, n2) o0) "([Hmy H1] & H2)".
-          iExists (n1,n2,Some o0).
-          iFrame.
-          iPoseProof (bi.and_elim_l with "H2") as "H3".
-          iPoseProof (bi.and_elim_r with "H3") as "Hnew".
+          iPoseProof (tree_rep_insert with "[$H1 $H2]") as "Hadd".
+          iDestruct "Hadd" as (r o0) "([Hmy H1] & H2)".
+          iExists (r, Some o0). iFrame. iDestruct "H2" as "[[Hnew _] _]".
           iIntros "H"; iDestruct "H" as %Hsub.
           iMod "Hnew".
-          iSpecialize ("Hnew" $! g1 g2).
+          iDestruct "Hnew" as (g1 g2) "H".
           iModIntro.
-          iExists (n1,n2, Some (Some(x,v,g1,g2))).
-          apply node_info_incl' in Hsub as [? Heq].
-          rewrite H5 in Heq.
-          inv Heq.
-          iExists (n1,n2, Some (Some (x,v,g1,g2))).
-          logic_to_iris.
-          instantiate (1 := v).
-          instantiate (1:= x).
-          iSplit.
+          iExists (r, Some (Some(x, v, g1, g2))).
+          iExists (r, Some (Some (x, v, g1, g2))).
+          apply node_info_incl' in Hsub as [? Heq]. simpl snd in *. inv Heq.
+          logic_to_iris. iSplit.
           {
-            iPureIntro. intros ? Hincl.
-            hnf. simpl. destruct (range_incl_join _ _ _ Hincl).
+            iPureIntro.
+            intros ? Hincl.
+            destruct b0 as ((n3, n4), i).
+            hnf.
+            simpl.
+            destruct (range_incl_join _ _ _ Hincl).
             simpl in *; subst. split; [|reflexivity].
-            split. { symmetry; rewrite merge_comm; apply merge_range_incl'; auto. }
-            destruct b0, Hincl as [_ Hincl]; simpl in Hincl. inv Hincl; try constructor.
-            simpl. inv H14.
+            split.
+            { symmetry; rewrite puretree.merge_comm; apply merge_range_incl'; auto. }
+            destruct Hincl as [_ Hincl]; simpl in Hincl.
+            inv Hincl; try constructor.
+            inv H12.
           }
           iIntros "(H1 & H2)".
-          iSpecialize ("Hnew" with "[$H2 $Hmy]").
+          instantiate (1 := x).
+          instantiate (1:= v).
+          iSpecialize ("H" with "[$H2 $Hmy]").
           iSplit; auto.
           {
             iPureIntro.
-            split; [reflexivity|].
+            split; auto.
             eapply key_in_range_incl; eassumption.
           }
-          iModIntro.
-          iDestruct "Hnew" as "($ & H3)".
-          iSplit; [iExists tt; auto|].
-          iExists n1, n2; iFrame.
-          iSplit; last done; iPureIntro.
+          iDestruct "H" as "(((((? & ?) & ?) & ?) & ?) & ?)".
+          iModIntro. rewrite exp_sepcon1; iExists tt.
+          rewrite !exp_sepcon2; iExists g1.
+          rewrite !exp_sepcon2; iExists g2.
+          rewrite !exp_sepcon2; iExists r.1.
+          rewrite !exp_sepcon2; iExists r.2; destruct r; iFrame.
+          iPureIntro; split; auto.
           eapply key_in_range_incl; eassumption.
-      }
-      Intros n1 n2.
-      forward_call (lock_in, lsh2,
-                     node_lock_inv_pred gsh g p1 g_in lock_in,
-                     node_lock_inv gsh g p1 g_in lock_in).
-      {
-        lock_props.
-        unfold node_lock_inv at 3.
-        rewrite selflock_eq.
-        unfold node_lock_inv_pred at 1, sync_inv at 1.
-        Exists (n1, n2, Some(Some (x, v, g1, g2))).
-        rewrite node_rep_def.
-        Exists tp; cancel.
+        }
+        go_lower.
+        rewrite -> prop_true_andp; auto.
+        destruct pt as ((((pnt & p1') & p2') & lock1) & lock2).
+        simpl.
+        (* erewrite <-  field_at_share_join; eauto. *)
+        unfold_data_at (data_at _ _ _ p1').
+        unfold_data_at (data_at _ _ _ p2').
+        (*already added *)
+        assert_PROP (field_compatible t_struct_tree_t [] p1') by entailer !.
+        assert_PROP (field_compatible t_struct_tree_t [] p2') by entailer !.
+        (**)
+        setoid_rewrite <- field_at_share_join with (p:= p1') at 2 ; eauto.
+        setoid_rewrite <- field_at_share_join with (p:= p2') at 2 ; eauto.
         unfold tree_rep_R.
-        rewrite -> if_false by auto.
-        Exists g1 g2 x v p1' p2' l1 l2.
-        unfold node_lock_inv; entailer!.
+        rewrite -> if_true; auto.
+        eapply derives_trans. apply fupd_frame_r.
+        apply  fupd_mono.
+        (* do Iris here to have pieces of things we need *)
+        iIntros "[[H1 H2] H2x]".
+        iDestruct "H2" as (g1 g2 n1 n2) "((((((%H2y & H3) & H4) & H5) & H6) & H7) & H8)".
+        iDestruct "H2x" as "(G1 & (G2 & (G3 & (G4 &
+                (G5 & (G6 & (G7 & (G8 & (G9 & (G10 &
+                (G11 & (G12 & (_ & (G14 & (G15 &
+                (G16 & (G17 & (G18 & (G19 & G20)))))))))))))))))))".
+        iDestruct "G10" as "(G10x & G10y & G10z)".
+        iDestruct "G11" as "(G11x & G11y & G11z)".
+        iAssert (node_lock_inv_pred gsh1 g p1' g1 lock1) with "[G10x G10z G5 H5 H7]" as "HRLock1".
+        {
+          unfold node_lock_inv_pred, sync_inv; auto.
+          iFrame.
+          iExists (n1, Finite_Integer x, Some None).
+          iFrame.
+          rewrite node_rep_def.
+          iExists nullval.
+          unfold tree_rep_R.
+          rewrite -> if_true; auto.
+          iFrame; done.
+        }
+        iAssert (node_lock_inv_pred gsh1 g p2' g2 lock2) with "[G11x G11z G6 H6 H8]" as "HRLock2".
+        {
+          unfold node_lock_inv_pred, sync_inv; auto.
+          iFrame.
+          iExists (Finite_Integer x, n2, Some None).
+          iFrame.
+          rewrite node_rep_def.
+          iExists nullval.
+          unfold tree_rep_R.
+          rewrite -> if_true; auto.
+          iFrame; done.
+        }
+        iAssert (|={⊤}=>
+                   (EX plock1, !!(ptr_of plock1 = lock1 /\ name_of plock1 = nroot .@ "Nlock1") &&
+                              lock_inv lsh1 plock1 (node_lock_inv gsh1 g p1' g1 plock1) ∗
+                        EX plock2, !!(ptr_of plock2 = lock2 /\ name_of plock2 = nroot .@ "Nlock2") &&
+                              lock_inv lsh1 plock2 (node_lock_inv gsh1 g p2' g2 plock2)))
+          with "[G7 G8 HRLock1 HRLock2]" as "HRL".
+        {
+          Intros. iVST.
+          rewrite <- 2sepcon_assoc.
+          eapply derives_trans
+            with (Q := |={⊤}=>(EX plock1 : lock_handle,
+                                 !! (ptr_of plock1 = lock1 ∧ name_of plock1 = nroot.@"Nlock1") &&
+                                   lock_inv lsh1 plock1 (node_lock_inv gsh1 g p1' g1 plock1)) *
+                               (EX plock2 : lock_handle,
+                                  !! (ptr_of plock2 = lock2 ∧ name_of plock2 = nroot.@"Nlock2") &&
+                                     lock_inv lsh1 plock2 (node_lock_inv gsh1 g p2' g2 plock2))).
+          iIntros "(((H1x & H1y) & H2) & H3)".
+          iSplitL "H1x H2".
+          Intros. iVST.
+          unfold node_lock_inv.
+          eapply derives_trans.
+          eapply make_lock_inv_0_self with (sh1 := lsh1) (sh2 := lsh2) (N := nroot .@ "Nlock1").
+          { apply readable_not_bot, readable_lsh1. }
+          eapply lsh1_lsh2_join.
+          eapply derives_trans, fupd_mono with
+          (P := EX h : lock_handle, !! (ptr_of h = lock1 ∧ name_of h = nroot.@"Nlock1") &&
+                                      lock_inv lsh1 h (node_lock_inv_pred gsh1 g p1' g1 lock1 *
+                                                         self_part lsh2 h)).
+          entailer !.
+          iIntros  "H".
+          iDestruct "H" as (l1) "H".
+          iExists l1.
+          unfold node_lock_inv.
+          Intros. iVST.
+          rewrite pull_left_special0.
+          entailer !.
+          Intros. iVST.
+          eapply derives_trans.
+          apply make_lock_inv_0_self with (sh1 := lsh1) (sh2 := lsh2) (N := nroot .@ "Nlock2").
+          { apply readable_not_bot, readable_lsh1. }
+          eapply lsh1_lsh2_join.
+          eapply derives_trans, fupd_mono
+            with (P := EX h : lock_handle, !! (ptr_of h = lock2 ∧ name_of h = nroot.@"Nlock2") &&
+                                      lock_inv lsh1 h (node_lock_inv_pred gsh1 g p2' g2 lock2 *
+                                                         self_part lsh2 h)).
+          entailer !.
+          iIntros  "H".
+          iDestruct "H" as (l2) "H".
+          iExists l2.
+          unfold node_lock_inv.
+          Intros. iVST.
+          rewrite pull_left_special0.
+          entailer !.
+          entailer !.
+        }
+        unfold node_lock_inv_new.
+        iFrame.
+        iIntros. iVST.
+        rewrite <- 10sepcon_comm; rewrite <- 10sepcon_assoc.
+        iIntros "((H & H1) & H2)".
+        iIntros. iVST.
+        rewrite <- sepcon_assoc.
+        rewrite -> sepcon_comm.
+        iIntros "H1".
+        iPoseProof (fupd_frame_r with "[$H1]") as "H1".
+        iApply (fupd_mono with "H1").
+        iIntros "((H1 & H2) & H3)".
+        iDestruct "H1" as (plock1) "[%H1x H1y]".
+        iDestruct "H2" as (plock2) "[%H2x H2y]".
+        iExists (true, (p1, (pnt, (lock_in, (gsh, (g_in, (n1, n2, Some (Some (x, v, g1, g2))))))))).
+        simpl.
+        iDestruct "H3" as "((((((G2 & G3) & G4) & G5) & G6) & G7) & G8)".
+        iDestruct "G2" as "((((K1 & K2) & K3) & K4) & K5)".
+        iSplit; try done.
+        iFrame.
+        unfold tree_rep_R.
+        simpl in H6.
+        rewrite -> if_false; auto.
+        iExists g1, g2, x, v, p1', p2', plock1, plock2.
+        unfold ltree.
+        iFrame.
+        Intros. iVST.
+        assert_PROP (is_pointer_or_null p1') by entailer !.
+        assert_PROP (is_pointer_or_null p2') by entailer !.
+        entailer !.
+        iIntros "H".
+        iApply (bi.later_sep_1).
+        iModIntro.
+        Intros. iVST.
+        destruct H1x.
+        destruct H2x.
+        rewrite H4.
+        rewrite H16.
+        entailer !.
+        repeat split; auto.
+      + repeat (match goal with |-context[|={⊤}=> ?P] => viewshift_SEP 0 P by entailer! end).
+        change emp with seplog.emp.
+        Intros pt.
+        destruct pt as (fl2 & (p2 & (tp2 & (lock_in2 & (gsh2 & (g_in2 & r2)))))).
+        unfold node_lock_inv_new.
+        simpl.
+        Intros.
+        forward.
+        forward.
+        (* _release2(_t'4) *)
+        unfold tree_rep_R.
+        rewrite if_false; auto.
+        Intros g1 g2 x1 v1 p1' p2' l1 l2.
+        assert_PROP (tp2 <> nullval) by entailer !.
+        (*  (_release2(_t'4); *)
+        forward_call release_self (lsh2, lock_in2,
+                    node_lock_inv_pred gsh2 g p2 g_in2 (ptr_of lock_in2)).
+        {
+          unfold node_lock_inv.
+          cancel.
+          unfold node_lock_inv_pred at 2.
+          unfold sync_inv.
+          destruct r2 as [p o].
+          simpl in H7, H10.
+          destruct p as [n1 n2].
+          Exists (n1, n2, Some (Some(x1, v1, g1, g2))).
+          rewrite node_rep_def.
+          Exists tp2; cancel.
+          unfold tree_rep_R. 
+          assert_PROP (tp2 <> nullval) by entailer!.
+          rewrite -> if_false by auto.
+          Exists g1 g2 x1 v1 p1' p2' l1 l2.
+          unfold ltree.
+          entailer !.
+          rewrite <- later_sepcon.
+          eapply derives_trans;
+              [|apply sepcon_derives, derives_refl; apply now_later].
+          entailer !.
+        }
+        forward_call (t_struct_pn, nb, gv).
+        { assert_PROP (nb <> nullval) by entailer !. rewrite if_false; auto. cancel. }
+        unfold nodebox_rep.
+        entailer !.
+        Exists np.
+        unfold ltree, node_lock_inv.
+        entailer !.
+      - (* (_t'6->_value) = _value;) *)
+        forward_if (
+            PROP ( )
+              LOCAL (temp _t'2 Vfalse; temp _t'8 (ptr_of lock); temp _t'7 np; temp _t'9 np;
+                      temp _pn__2 nb; gvars gv; temp _t b; temp _x (vint x); temp _value v)
+              SEP (Q1 (false, (p1, (tp, (lock_in, (gsh, (g_in, (x0, r)))))));
+                    mem_mgr gv; seplog.emp;
+                    field_at Ews t_struct_tree_t (DOT _t) tp p1 *
+                      malloc_token Ews t_struct_tree_t p1 * in_tree g g_in *
+                      (EX (ga gb : gname) (x1 : Z) (v0 pa pb : val) (locka lockb : lock_handle),
+                        !! ((x0, r).2 = Some (Some (x1, v0, ga, gb))
+                            ∧ (Int.min_signed ≤ x1 ≤ Int.max_signed)%Z
+                            ∧ is_pointer_or_null pa
+                            ∧ is_pointer_or_null pb ∧ tc_val (tptr Tvoid) v0 ∧
+                              key_in_range x1 (x0, r).1 = true) &&
+                          data_at Ews t_struct_tree (vint x1, (v, (pa, pb))) tp *
+                          malloc_token Ews t_struct_tree tp *
+                          |> ltree g ga lsh1 gsh1 pa locka *
+                          |> ltree g gb lsh1 gsh1 pb lockb) *
+                      my_half g_in gsh (x0, r) *
+                      field_at lsh2 t_struct_tree_t (DOT _lock) (ptr_of lock_in) p1 *
+                      |> lock_inv lsh2 lock_in (node_lock_inv gsh g p1 g_in lock_in);
+                    data_at Ews t_struct_pn (p1, p1) nb;
+                    my_half g_root (Share.split gsh1).2 (Neg_Infinity, Pos_Infinity, None);
+                    data_at sh (tptr t_struct_tree_t) np b;
+                    field_at sh t_struct_tree_t (DOT _lock) (ptr_of lock) np;
+                    lock_inv sh lock (node_lock_inv (Share.split gsh1).1 g np g_root lock);
+                    malloc_token Ews t_struct_pn nb)).
+        + destruct H3 as ( ?  & v2 & g21 & g22 & ?).
+          unfold node_lock_inv_new, tree_rep_R.
+          rewrite -> if_false; auto.
+          simpl in *.
+          Intros g1 g2 x1 v1 p1' p2' l1 l2.
+          forward.
+          forward.
+          forward.
+          Exists g1 g2 x1 v1 p1' p2' l1 l2.
+          entailer !.
+      + (* contradiction, since  Int.one = Int.zero *)
+        pose proof Int.one_not_zero; contradiction.
+      + autorewrite with norm.
+        destruct H3 as ( ? & v2 & g21 & g22 & ?).
+        Intros g1 g2 x1 v1 p1' p2' l1 l2.
+        forward.
+        forward.
+        simpl in H5. rewrite H5 in H4. injection H4.
+        intros. subst x1. subst v2. subst g21. subst g22.
+        unfold Q1.
+        simpl.
+        gather_SEP AS (my_half g_in _ _) (in_tree g  _).
+        viewshift_SEP 0 (Q *
+                    (EX n1 n2:number,
+                      !!(key_in_range x (n1,n2) = true) 
+                      && my_half g_in gsh (n1,n2,Some (Some(x,v,g1,g2))) * in_tree g g_in)).
+        {
+            go_lower.
+            eapply sync_commit_gen1.
+            intros. iIntros "H".
+            iDestruct "H" as "[H1 H2]".
+            iModIntro.
+            iPoseProof (tree_rep_insert x1 g g_root g_in with "[H1 H2]") as "Hadd".
+            iSplitL "H2"; auto.
+            iDestruct "Hadd" as ((n1, n2) o0) "([Hmy H1] & H2)".
+            iExists (n1,n2,Some o0).
+            iSplitL "H1". iFrame.
+            iPoseProof (bi.and_elim_l with "H2") as "H3".
+            iPoseProof (bi.and_elim_r with "H3") as "Hnew".
+            iIntros "H". iDestruct "H" as %Hsub.
+            iMod "Hnew".
+            iSpecialize ("Hnew" $! g1 g2).
+            iModIntro.
+            iExists (n1,n2, Some (Some(x,v,g1,g2))).
+            apply node_info_incl' in Hsub as [? Heq].
+            rewrite H5 in Heq.
+            inv Heq.
+            iExists (n1,n2, Some (Some (x,v,g1,g2))).
+            logic_to_iris.
+            instantiate (1 := v).
+            instantiate (1:= x).
+            iSplit.
+            {
+              iPureIntro. intros ? Hincl.
+              hnf. simpl. destruct (range_incl_join _ _ _ Hincl).
+              simpl in *; subst. split; [|reflexivity].
+              split.
+              { symmetry.
+                rewrite puretree.merge_comm; apply merge_range_incl'; auto. }
+              destruct b0, Hincl as [_ Hincl]; simpl in Hincl. inv Hincl; try constructor.
+              simpl. inv H16.
+            }
+            iIntros "(H1 & H2)".
+            iSpecialize ("Hnew" $! v1 with "[$H2 $Hmy]").
+            iSplit; auto.
+            {
+              iPureIntro.
+              split; [reflexivity|].
+              eapply key_in_range_incl; eassumption.
+            }
+            iModIntro.
+            iDestruct "Hnew" as "($ & H3)".
+            iSplit; [iExists tt; auto|].
+            iExists n1, n2; iFrame.
+            iSplit; last done; iPureIntro.
+            eapply key_in_range_incl; eassumption.
+        }
+        Intros n1 n2.
+        unfold ltree.
+        Intros.
+        forward_call release_self (lsh2, lock_in,
+                      node_lock_inv_pred gsh g p1 g_in (ptr_of lock_in)).
+        {
+          unfold node_lock_inv.
+          entailer !.
+          unfold node_lock_inv_pred at 4.
+          unfold sync_inv.
+          Exists (n1, n2, Some(Some (x, v, g1, g2))).
+          rewrite node_rep_def.
+          Exists tp; cancel.
+          unfold tree_rep_R.
+          rewrite -> if_false by auto.
+          Exists g1 g2 x v p1' p2' l1 l2.
+          unfold ltree.
+          entailer !.
+          rewrite <- later_sepcon;
+            eapply derives_trans;
+            [|apply sepcon_derives, derives_refl; apply now_later].
+          entailer !.
+        }
+        forward_call (t_struct_pn, nb, gv).
+        { assert_PROP (nb <> nullval) by entailer !. rewrite if_false; auto. cancel. }
+        unfold nodebox_rep.
+        entailer !.
+        Exists np.
+        cancel.
+        unfold ltree, node_lock_inv.
+        entailer !.
       }
-      forward_call (t_struct_pn, nb, gv).
-      {
-       assert_PROP (nb <> nullval) by entailer !.
-       rewrite if_false; auto.
-       cancel.
-      }
-      unfold nodebox_rep.
-      entailer !.
-      Exists np.
-      unfold ltree, node_lock_inv.
-      entailer !.
 Qed.
-
-
