concurrency/bst_template.v
@@ -15,7 +15,7 @@ Module Info.
   Definition abi := "macos".
   Definition bitsize := 64.
   Definition big_endian := false.
-  Definition source_file := "bst_template.c".
+  Definition source_file := "main.c".
   Definition normalized := true.
 End Info.
 
@@ -83,16 +83,15 @@ Definition ___stringlit_5 : ident := $"__stringlit_5".
 Definition ___stringlit_6 : ident := $"__stringlit_6".
 Definition ___stringlit_7 : ident := $"__stringlit_7".
 Definition ___stringlit_8 : ident := $"__stringlit_8".
-Definition ___stringlit_9 : ident := $"__stringlit_9".
 Definition _acquire : ident := $"acquire".
 Definition _args : ident := $"args".
+Definition _atom_int : ident := $"atom_int".
 Definition _b : ident := $"b".
 Definition _exit : ident := $"exit".
 Definition _findnext : ident := $"findnext".
 Definition _flag : ident := $"flag".
 Definition _free : ident := $"free".
-Definition _freelock2 : ident := $"freelock2".
-Definition _insert : ident := $"insert".
+Definition _freelock : ident := $"freelock".
 Definition _insert2 : ident := $"insert2".
 Definition _insertOp : ident := $"insertOp".
 Definition _key : ident := $"key".
@@ -117,7 +116,7 @@ Definition _pb : ident := $"pb".
 Definition _pn : ident := $"pn".
 Definition _pn__2 : ident := $"pn__2".
 Definition _printf : ident := $"printf".
-Definition _release2 : ident := $"release2".
+Definition _release : ident := $"release".
 Definition _right : ident := $"right".
 Definition _spawn : ident := $"spawn".
 Definition _surely_malloc : ident := $"surely_malloc".
@@ -127,7 +126,6 @@ Definition _tb : ident := $"tb".
 Definition _tgp : ident := $"tgp".
 Definition _tgt : ident := $"tgt".
 Definition _thread_func : ident := $"thread_func".
-Definition _thread_lock : ident := $"thread_lock".
 Definition _traverse : ident := $"traverse".
 Definition _traverseInorder : ident := $"traverseInorder".
 Definition _tree : ident := $"tree".
@@ -154,7 +152,7 @@ Definition _t'7 : ident := 134%positive.
 Definition _t'8 : ident := 135%positive.
 Definition _t'9 : ident := 136%positive.
 
-Definition v___stringlit_7 := {|
+Definition v___stringlit_6 := {|
   gvar_info := (tarray tschar 5);
   gvar_init := (Init_int8 (Int.repr 102) :: Init_int8 (Int.repr 111) ::
                 Init_int8 (Int.repr 117) :: Init_int8 (Int.repr 114) ::
@@ -163,7 +161,7 @@ Definition v___stringlit_7 := {|
   gvar_volatile := false
 |}.
 
-Definition v___stringlit_5 := {|
+Definition v___stringlit_4 := {|
   gvar_info := (tarray tschar 6);
   gvar_init := (Init_int8 (Int.repr 116) :: Init_int8 (Int.repr 104) ::
                 Init_int8 (Int.repr 114) :: Init_int8 (Int.repr 101) ::
@@ -172,25 +170,7 @@ Definition v___stringlit_5 := {|
   gvar_volatile := false
 |}.
 
-Definition v___stringlit_2 := {|
-  gvar_info := (tarray tschar 24);
-  gvar_init := (Init_int8 (Int.repr 82) :: Init_int8 (Int.repr 105) ::
-                Init_int8 (Int.repr 103) :: Init_int8 (Int.repr 104) ::
-                Init_int8 (Int.repr 116) :: Init_int8 (Int.repr 32) ::
-                Init_int8 (Int.repr 45) :: Init_int8 (Int.repr 32) ::
-                Init_int8 (Int.repr 120) :: Init_int8 (Int.repr 32) ::
-                Init_int8 (Int.repr 61) :: Init_int8 (Int.repr 32) ::
-                Init_int8 (Int.repr 37) :: Init_int8 (Int.repr 100) ::
-                Init_int8 (Int.repr 44) :: Init_int8 (Int.repr 32) ::
-                Init_int8 (Int.repr 121) :: Init_int8 (Int.repr 32) ::
-                Init_int8 (Int.repr 61) :: Init_int8 (Int.repr 32) ::
-                Init_int8 (Int.repr 37) :: Init_int8 (Int.repr 100) ::
-                Init_int8 (Int.repr 10) :: Init_int8 (Int.repr 0) :: nil);
-  gvar_readonly := true;
-  gvar_volatile := false
-|}.
-
-Definition v___stringlit_4 := {|
+Definition v___stringlit_1 := {|
   gvar_info := (tarray tschar 19);
   gvar_init := (Init_int8 (Int.repr 110) :: Init_int8 (Int.repr 111) ::
                 Init_int8 (Int.repr 100) :: Init_int8 (Int.repr 101) ::
@@ -206,25 +186,7 @@ Definition v___stringlit_4 := {|
   gvar_volatile := false
 |}.
 
-Definition v___stringlit_3 := {|
-  gvar_info := (tarray tschar 23);
-  gvar_init := (Init_int8 (Int.repr 76) :: Init_int8 (Int.repr 101) ::
-                Init_int8 (Int.repr 102) :: Init_int8 (Int.repr 116) ::
-                Init_int8 (Int.repr 32) :: Init_int8 (Int.repr 45) ::
-                Init_int8 (Int.repr 32) :: Init_int8 (Int.repr 120) ::
-                Init_int8 (Int.repr 32) :: Init_int8 (Int.repr 61) ::
-                Init_int8 (Int.repr 32) :: Init_int8 (Int.repr 37) ::
-                Init_int8 (Int.repr 100) :: Init_int8 (Int.repr 44) ::
-                Init_int8 (Int.repr 32) :: Init_int8 (Int.repr 121) ::
-                Init_int8 (Int.repr 32) :: Init_int8 (Int.repr 61) ::
-                Init_int8 (Int.repr 32) :: Init_int8 (Int.repr 37) ::
-                Init_int8 (Int.repr 100) :: Init_int8 (Int.repr 10) ::
-                Init_int8 (Int.repr 0) :: nil);
-  gvar_readonly := true;
-  gvar_volatile := false
-|}.
-
-Definition v___stringlit_9 := {|
+Definition v___stringlit_8 := {|
   gvar_info := (tarray tschar 10);
   gvar_init := (Init_int8 (Int.repr 84) :: Init_int8 (Int.repr 114) ::
                 Init_int8 (Int.repr 97) :: Init_int8 (Int.repr 118) ::
@@ -235,21 +197,21 @@ Definition v___stringlit_9 := {|
   gvar_volatile := false
 |}.
 
-Definition v___stringlit_1 := {|
-  gvar_info := (tarray tschar 15);
-  gvar_init := (Init_int8 (Int.repr 69) :: Init_int8 (Int.repr 120) ::
-                Init_int8 (Int.repr 99) :: Init_int8 (Int.repr 108) ::
-                Init_int8 (Int.repr 117) :: Init_int8 (Int.repr 100) ::
-                Init_int8 (Int.repr 101) :: Init_int8 (Int.repr 32) ::
-                Init_int8 (Int.repr 37) :: Init_int8 (Int.repr 100) ::
-                Init_int8 (Int.repr 32) :: Init_int8 (Int.repr 37) ::
-                Init_int8 (Int.repr 115) :: Init_int8 (Int.repr 10) ::
-                Init_int8 (Int.repr 0) :: nil);
+Definition v___stringlit_2 := {|
+  gvar_info := (tarray tschar 16);
+  gvar_init := (Init_int8 (Int.repr 79) :: Init_int8 (Int.repr 78) ::
+                Init_int8 (Int.repr 69) :: Init_int8 (Int.repr 95) ::
+                Init_int8 (Int.repr 70) :: Init_int8 (Int.repr 82) ::
+                Init_int8 (Int.repr 79) :: Init_int8 (Int.repr 77) ::
+                Init_int8 (Int.repr 95) :: Init_int8 (Int.repr 84) ::
+                Init_int8 (Int.repr 72) :: Init_int8 (Int.repr 82) ::
+                Init_int8 (Int.repr 69) :: Init_int8 (Int.repr 65) ::
+                Init_int8 (Int.repr 68) :: Init_int8 (Int.repr 0) :: nil);
   gvar_readonly := true;
   gvar_volatile := false
 |}.
 
-Definition v___stringlit_8 := {|
+Definition v___stringlit_7 := {|
   gvar_info := (tarray tschar 4);
   gvar_init := (Init_int8 (Int.repr 37) :: Init_int8 (Int.repr 115) ::
                 Init_int8 (Int.repr 10) :: Init_int8 (Int.repr 0) :: nil);
@@ -257,7 +219,7 @@ Definition v___stringlit_8 := {|
   gvar_volatile := false
 |}.
 
-Definition v___stringlit_6 := {|
+Definition v___stringlit_5 := {|
   gvar_info := (tarray tschar 4);
   gvar_init := (Init_int8 (Int.repr 79) :: Init_int8 (Int.repr 110) ::
                 Init_int8 (Int.repr 101) :: Init_int8 (Int.repr 0) :: nil);
@@ -265,10 +227,12 @@ Definition v___stringlit_6 := {|
   gvar_volatile := false
 |}.
 
-Definition v_thread_lock := {|
-  gvar_info := (tarray (tptr tvoid) 2);
-  gvar_init := (Init_space 16 :: nil);
-  gvar_readonly := false;
+Definition v___stringlit_3 := {|
+  gvar_info := (tarray tschar 5);
+  gvar_init := (Init_int8 (Int.repr 70) :: Init_int8 (Int.repr 79) ::
+                Init_int8 (Int.repr 85) :: Init_int8 (Int.repr 82) ::
+                Init_int8 (Int.repr 0) :: nil);
+  gvar_readonly := true;
   gvar_volatile := false
 |}.
 
@@ -307,9 +271,9 @@ Definition f_treebox_new := {|
   fn_vars := nil;
   fn_temps := ((_p, (tptr (tptr (Tstruct _tree_t noattr)))) ::
                (_newt, (tptr (Tstruct _tree_t noattr))) ::
-               (_l, (tptr (tarray (tptr tvoid) 2))) ::
-               (_t'3, (tptr tvoid)) :: (_t'2, (tptr tvoid)) ::
-               (_t'1, (tptr tvoid)) :: nil);
+               (_l, (tptr (Tstruct _atom_int noattr))) ::
+               (_t'3, (tptr (Tstruct _atom_int noattr))) ::
+               (_t'2, (tptr tvoid)) :: (_t'1, (tptr tvoid)) :: nil);
   fn_body :=
 (Ssequence
   (Ssequence
@@ -336,37 +300,29 @@ Definition f_treebox_new := {|
       (Ssequence
         (Ssequence
           (Scall (Some _t'3)
-            (Evar _surely_malloc (Tfunction (Tcons tulong Tnil) (tptr tvoid)
-                                   cc_default))
-            ((Esizeof (tarray (tptr tvoid) 2) tulong) :: nil))
-          (Sset _l
-            (Ecast (Etempvar _t'3 (tptr tvoid))
-              (tptr (tarray (tptr tvoid) 2)))))
+            (Evar _makelock (Tfunction Tnil (tptr (Tstruct _atom_int noattr))
+                              cc_default)) nil)
+          (Sset _l (Etempvar _t'3 (tptr (Tstruct _atom_int noattr)))))
         (Ssequence
-          (Scall None
-            (Evar _makelock (Tfunction (Tcons (tptr tvoid) Tnil) tvoid
-                              cc_default))
-            ((Etempvar _l (tptr (tarray (tptr tvoid) 2))) :: nil))
+          (Sassign
+            (Efield
+              (Ederef (Etempvar _newt (tptr (Tstruct _tree_t noattr)))
+                (Tstruct _tree_t noattr)) _lock
+              (tptr (Tstruct _atom_int noattr)))
+            (Etempvar _l (tptr (Tstruct _atom_int noattr))))
           (Ssequence
             (Sassign
               (Efield
                 (Ederef (Etempvar _newt (tptr (Tstruct _tree_t noattr)))
-                  (Tstruct _tree_t noattr)) _lock
-                (tptr (tarray (tptr tvoid) 2)))
-              (Etempvar _l (tptr (tarray (tptr tvoid) 2))))
+                  (Tstruct _tree_t noattr)) _t (tptr (Tstruct _tree noattr)))
+              (Ecast (Econst_int (Int.repr 0) tint) (tptr tvoid)))
             (Ssequence
-              (Sassign
-                (Efield
-                  (Ederef (Etempvar _newt (tptr (Tstruct _tree_t noattr)))
-                    (Tstruct _tree_t noattr)) _t
-                  (tptr (Tstruct _tree noattr)))
-                (Ecast (Econst_int (Int.repr 0) tint) (tptr tvoid)))
-              (Ssequence
-                (Scall None
-                  (Evar _release2 (Tfunction (Tcons (tptr tvoid) Tnil) tvoid
-                                    cc_default))
-                  ((Etempvar _l (tptr (tarray (tptr tvoid) 2))) :: nil))
-                (Sreturn (Some (Etempvar _p (tptr (tptr (Tstruct _tree_t noattr))))))))))))))
+              (Scall None
+                (Evar _release (Tfunction
+                                 (Tcons (tptr (Tstruct _atom_int noattr))
+                                   Tnil) tvoid cc_default))
+                ((Etempvar _l (tptr (Tstruct _atom_int noattr))) :: nil))
+              (Sreturn (Some (Etempvar _p (tptr (tptr (Tstruct _tree_t noattr)))))))))))))
 |}.
 
 Definition f_tree_free := {|
@@ -383,11 +339,12 @@ Definition f_tree_free := {|
   (Sset _l
     (Efield
       (Ederef (Etempvar _tgp (tptr (Tstruct _tree_t noattr)))
-        (Tstruct _tree_t noattr)) _lock (tptr (tarray (tptr tvoid) 2))))
+        (Tstruct _tree_t noattr)) _lock (tptr (Tstruct _atom_int noattr))))
   (Ssequence
     (Scall None
-      (Evar _acquire (Tfunction (Tcons (tptr tvoid) Tnil) tvoid cc_default))
-      ((Etempvar _l (tptr tvoid)) :: nil))
+      (Evar _acquire (Tfunction
+                       (Tcons (tptr (Tstruct _atom_int noattr)) Tnil) tvoid
+                       cc_default)) ((Etempvar _l (tptr tvoid)) :: nil))
     (Ssequence
       (Sset _p
         (Efield
@@ -428,8 +385,9 @@ Definition f_tree_free := {|
           Sskip)
         (Ssequence
           (Scall None
-            (Evar _freelock2 (Tfunction (Tcons (tptr tvoid) Tnil) tvoid
-                               cc_default))
+            (Evar _freelock (Tfunction
+                              (Tcons (tptr (Tstruct _atom_int noattr)) Tnil)
+                              tvoid cc_default))
             ((Etempvar _l (tptr tvoid)) :: nil))
           (Ssequence
             (Scall None
@@ -461,344 +419,6 @@ Definition f_treebox_free := {|
     (Scall None
       (Evar _free (Tfunction (Tcons (tptr tvoid) Tnil) tvoid cc_default))
       ((Etempvar _b (tptr (tptr (Tstruct _tree_t noattr)))) :: nil))))
-|}.
-
-Definition f_insert := {|
-  fn_return := tvoid;
-  fn_callconv := cc_default;
-  fn_params := ((_t, (tptr (tptr (Tstruct _tree_t noattr)))) :: (_x, tint) ::
-                (_value, (tptr tvoid)) :: nil);
-  fn_vars := nil;
-  fn_temps := ((_tgt, (tptr (Tstruct _tree_t noattr))) ::
-               (_p, (tptr (Tstruct _tree noattr))) :: (_l, (tptr tvoid)) ::
-               (_p1, (tptr (Tstruct _tree_t noattr))) ::
-               (_p2, (tptr (Tstruct _tree_t noattr))) ::
-               (_l1, (tptr (tarray (tptr tvoid) 2))) ::
-               (_l2, (tptr (tarray (tptr tvoid) 2))) :: (_y, tint) ::
-               (_l_old, (tptr tvoid)) :: (_l_old__1, (tptr tvoid)) ::
-               (_t'5, (tptr tvoid)) :: (_t'4, (tptr tvoid)) ::
-               (_t'3, (tptr tvoid)) :: (_t'2, (tptr tvoid)) ::
-               (_t'1, (tptr tvoid)) :: (_t'9, tint) :: (_t'8, tint) ::
-               (_t'7, (tptr tvoid)) :: (_t'6, tint) :: nil);
-  fn_body :=
-(Ssequence
-  (Sset _tgt
-    (Ederef (Etempvar _t (tptr (tptr (Tstruct _tree_t noattr))))
-      (tptr (Tstruct _tree_t noattr))))
-  (Ssequence
-    (Sset _l
-      (Efield
-        (Ederef (Etempvar _tgt (tptr (Tstruct _tree_t noattr)))
-          (Tstruct _tree_t noattr)) _lock (tptr (tarray (tptr tvoid) 2))))
-    (Ssequence
-      (Scall None
-        (Evar _acquire (Tfunction (Tcons (tptr tvoid) Tnil) tvoid cc_default))
-        ((Etempvar _l (tptr tvoid)) :: nil))
-      (Sloop
-        (Ssequence
-          Sskip
-          (Ssequence
-            (Sset _p
-              (Efield
-                (Ederef (Etempvar _tgt (tptr (Tstruct _tree_t noattr)))
-                  (Tstruct _tree_t noattr)) _t (tptr (Tstruct _tree noattr))))
-            (Sifthenelse (Ebinop Oeq
-                           (Etempvar _p (tptr (Tstruct _tree noattr)))
-                           (Ecast (Econst_int (Int.repr 0) tint)
-                             (tptr tvoid)) tint)
-              (Ssequence
-                (Ssequence
-                  (Scall (Some _t'1)
-                    (Evar _surely_malloc (Tfunction (Tcons tulong Tnil)
-                                           (tptr tvoid) cc_default))
-                    ((Esizeof (Tstruct _tree_t noattr) tulong) :: nil))
-                  (Sset _p1
-                    (Ecast (Etempvar _t'1 (tptr tvoid))
-                      (tptr (Tstruct _tree_t noattr)))))
-                (Ssequence
-                  (Ssequence
-                    (Scall (Some _t'2)
-                      (Evar _surely_malloc (Tfunction (Tcons tulong Tnil)
-                                             (tptr tvoid) cc_default))
-                      ((Esizeof (Tstruct _tree_t noattr) tulong) :: nil))
-                    (Sset _p2
-                      (Ecast (Etempvar _t'2 (tptr tvoid))
-                        (tptr (Tstruct _tree_t noattr)))))
-                  (Ssequence
-                    (Sassign
-                      (Efield
-                        (Ederef
-                          (Etempvar _p1 (tptr (Tstruct _tree_t noattr)))
-                          (Tstruct _tree_t noattr)) _t
-                        (tptr (Tstruct _tree noattr)))
-                      (Ecast (Econst_int (Int.repr 0) tint) (tptr tvoid)))
-                    (Ssequence
-                      (Sassign
-                        (Efield
-                          (Ederef
-                            (Etempvar _p2 (tptr (Tstruct _tree_t noattr)))
-                            (Tstruct _tree_t noattr)) _t
-                          (tptr (Tstruct _tree noattr)))
-                        (Ecast (Econst_int (Int.repr 0) tint) (tptr tvoid)))
-                      (Ssequence
-                        (Ssequence
-                          (Scall (Some _t'3)
-                            (Evar _surely_malloc (Tfunction
-                                                   (Tcons tulong Tnil)
-                                                   (tptr tvoid) cc_default))
-                            ((Esizeof (tarray (tptr tvoid) 2) tulong) :: nil))
-                          (Sset _l1
-                            (Ecast (Etempvar _t'3 (tptr tvoid))
-                              (tptr (tarray (tptr tvoid) 2)))))
-                        (Ssequence
-                          (Scall None
-                            (Evar _makelock (Tfunction
-                                              (Tcons (tptr tvoid) Tnil) tvoid
-                                              cc_default))
-                            ((Etempvar _l1 (tptr (tarray (tptr tvoid) 2))) ::
-                             nil))
-                          (Ssequence
-                            (Sassign
-                              (Efield
-                                (Ederef
-                                  (Etempvar _p1 (tptr (Tstruct _tree_t noattr)))
-                                  (Tstruct _tree_t noattr)) _lock
-                                (tptr (tarray (tptr tvoid) 2)))
-                              (Etempvar _l1 (tptr (tarray (tptr tvoid) 2))))
-                            (Ssequence
-                              (Scall None
-                                (Evar _release2 (Tfunction
-                                                  (Tcons (tptr tvoid) Tnil)
-                                                  tvoid cc_default))
-                                ((Etempvar _l1 (tptr (tarray (tptr tvoid) 2))) ::
-                                 nil))
-                              (Ssequence
-                                (Ssequence
-                                  (Scall (Some _t'4)
-                                    (Evar _surely_malloc (Tfunction
-                                                           (Tcons tulong
-                                                             Tnil)
-                                                           (tptr tvoid)
-                                                           cc_default))
-                                    ((Esizeof (tarray (tptr tvoid) 2) tulong) ::
-                                     nil))
-                                  (Sset _l2
-                                    (Ecast (Etempvar _t'4 (tptr tvoid))
-                                      (tptr (tarray (tptr tvoid) 2)))))
-                                (Ssequence
-                                  (Scall None
-                                    (Evar _makelock (Tfunction
-                                                      (Tcons (tptr tvoid)
-                                                        Tnil) tvoid
-                                                      cc_default))
-                                    ((Etempvar _l2 (tptr (tarray (tptr tvoid) 2))) ::
-                                     nil))
-                                  (Ssequence
-                                    (Sassign
-                                      (Efield
-                                        (Ederef
-                                          (Etempvar _p2 (tptr (Tstruct _tree_t noattr)))
-                                          (Tstruct _tree_t noattr)) _lock
-                                        (tptr (tarray (tptr tvoid) 2)))
-                                      (Etempvar _l2 (tptr (tarray (tptr tvoid) 2))))
-                                    (Ssequence
-                                      (Scall None
-                                        (Evar _release2 (Tfunction
-                                                          (Tcons (tptr tvoid)
-                                                            Tnil) tvoid
-                                                          cc_default))
-                                        ((Etempvar _l2 (tptr (tarray (tptr tvoid) 2))) ::
-                                         nil))
-                                      (Ssequence
-                                        (Ssequence
-                                          (Scall (Some _t'5)
-                                            (Evar _surely_malloc (Tfunction
-                                                                   (Tcons
-                                                                    tulong
-                                                                    Tnil)
-                                                                   (tptr tvoid)
-                                                                   cc_default))
-                                            ((Esizeof (Tstruct _tree noattr) tulong) ::
-                                             nil))
-                                          (Sset _p
-                                            (Ecast
-                                              (Etempvar _t'5 (tptr tvoid))
-                                              (tptr (Tstruct _tree noattr)))))
-                                        (Ssequence
-                                          (Sassign
-                                            (Efield
-                                              (Ederef
-                                                (Etempvar _tgt (tptr (Tstruct _tree_t noattr)))
-                                                (Tstruct _tree_t noattr)) _t
-                                              (tptr (Tstruct _tree noattr)))
-                                            (Etempvar _p (tptr (Tstruct _tree noattr))))
-                                          (Ssequence
-                                            (Sassign
-                                              (Efield
-                                                (Ederef
-                                                  (Etempvar _p (tptr (Tstruct _tree noattr)))
-                                                  (Tstruct _tree noattr))
-                                                _key tint)
-                                              (Etempvar _x tint))
-                                            (Ssequence
-                                              (Sassign
-                                                (Efield
-                                                  (Ederef
-                                                    (Etempvar _p (tptr (Tstruct _tree noattr)))
-                                                    (Tstruct _tree noattr))
-                                                  _value (tptr tvoid))
-                                                (Etempvar _value (tptr tvoid)))
-                                              (Ssequence
-                                                (Sassign
-                                                  (Efield
-                                                    (Ederef
-                                                      (Etempvar _p (tptr (Tstruct _tree noattr)))
-                                                      (Tstruct _tree noattr))
-                                                    _left
-                                                    (tptr (Tstruct _tree_t noattr)))
-                                                  (Etempvar _p1 (tptr (Tstruct _tree_t noattr))))
-                                                (Ssequence
-                                                  (Sassign
-                                                    (Efield
-                                                      (Ederef
-                                                        (Etempvar _p (tptr (Tstruct _tree noattr)))
-                                                        (Tstruct _tree noattr))
-                                                      _right
-                                                      (tptr (Tstruct _tree_t noattr)))
-                                                    (Etempvar _p2 (tptr (Tstruct _tree_t noattr))))
-                                                  (Ssequence
-                                                    (Scall None
-                                                      (Evar _release2 
-                                                      (Tfunction
-                                                        (Tcons (tptr tvoid)
-                                                          Tnil) tvoid
-                                                        cc_default))
-                                                      ((Etempvar _l (tptr tvoid)) ::
-                                                       nil))
-                                                    (Sreturn None))))))))))))))))))))
-              (Ssequence
-                (Sset _y
-                  (Efield
-                    (Ederef (Etempvar _p (tptr (Tstruct _tree noattr)))
-                      (Tstruct _tree noattr)) _key tint))
-                (Sifthenelse (Ebinop Olt (Etempvar _x tint)
-                               (Etempvar _y tint) tint)
-                  (Ssequence
-                    (Sset _tgt
-                      (Efield
-                        (Ederef (Etempvar _p (tptr (Tstruct _tree noattr)))
-                          (Tstruct _tree noattr)) _left
-                        (tptr (Tstruct _tree_t noattr))))
-                    (Ssequence
-                      (Ssequence
-                        (Sset _t'9
-                          (Efield
-                            (Ederef
-                              (Etempvar _p (tptr (Tstruct _tree noattr)))
-                              (Tstruct _tree noattr)) _key tint))
-                        (Scall None
-                          (Evar _printf (Tfunction (Tcons (tptr tschar) Tnil)
-                                          tint
-                                          {|cc_vararg:=(Some 1); cc_unproto:=false; cc_structret:=false|}))
-                          ((Evar ___stringlit_3 (tarray tschar 23)) ::
-                           (Etempvar _x tint) :: (Etempvar _t'9 tint) :: nil)))
-                      (Ssequence
-                        (Sset _l_old (Etempvar _l (tptr tvoid)))
-                        (Ssequence
-                          (Sset _l
-                            (Efield
-                              (Ederef
-                                (Etempvar _tgt (tptr (Tstruct _tree_t noattr)))
-                                (Tstruct _tree_t noattr)) _lock
-                              (tptr (tarray (tptr tvoid) 2))))
-                          (Ssequence
-                            (Scall None
-                              (Evar _acquire (Tfunction
-                                               (Tcons (tptr tvoid) Tnil)
-                                               tvoid cc_default))
-                              ((Etempvar _l (tptr tvoid)) :: nil))
-                            (Scall None
-                              (Evar _release2 (Tfunction
-                                                (Tcons (tptr tvoid) Tnil)
-                                                tvoid cc_default))
-                              ((Etempvar _l_old (tptr tvoid)) :: nil)))))))
-                  (Sifthenelse (Ebinop Olt (Etempvar _y tint)
-                                 (Etempvar _x tint) tint)
-                    (Ssequence
-                      (Sset _tgt
-                        (Efield
-                          (Ederef (Etempvar _p (tptr (Tstruct _tree noattr)))
-                            (Tstruct _tree noattr)) _right
-                          (tptr (Tstruct _tree_t noattr))))
-                      (Ssequence
-                        (Ssequence
-                          (Sset _t'8
-                            (Efield
-                              (Ederef
-                                (Etempvar _p (tptr (Tstruct _tree noattr)))
-                                (Tstruct _tree noattr)) _key tint))
-                          (Scall None
-                            (Evar _printf (Tfunction
-                                            (Tcons (tptr tschar) Tnil) tint
-                                            {|cc_vararg:=(Some 1); cc_unproto:=false; cc_structret:=false|}))
-                            ((Evar ___stringlit_2 (tarray tschar 24)) ::
-                             (Etempvar _x tint) :: (Etempvar _t'8 tint) ::
-                             nil)))
-                        (Ssequence
-                          (Sset _l_old__1 (Etempvar _l (tptr tvoid)))
-                          (Ssequence
-                            (Sset _l
-                              (Efield
-                                (Ederef
-                                  (Etempvar _tgt (tptr (Tstruct _tree_t noattr)))
-                                  (Tstruct _tree_t noattr)) _lock
-                                (tptr (tarray (tptr tvoid) 2))))
-                            (Ssequence
-                              (Scall None
-                                (Evar _acquire (Tfunction
-                                                 (Tcons (tptr tvoid) Tnil)
-                                                 tvoid cc_default))
-                                ((Etempvar _l (tptr tvoid)) :: nil))
-                              (Scall None
-                                (Evar _release2 (Tfunction
-                                                  (Tcons (tptr tvoid) Tnil)
-                                                  tvoid cc_default))
-                                ((Etempvar _l_old__1 (tptr tvoid)) :: nil)))))))
-                    (Ssequence
-                      (Sassign
-                        (Efield
-                          (Ederef (Etempvar _p (tptr (Tstruct _tree noattr)))
-                            (Tstruct _tree noattr)) _value (tptr tvoid))
-                        (Etempvar _value (tptr tvoid)))
-                      (Ssequence
-                        (Ssequence
-                          (Sset _t'6
-                            (Efield
-                              (Ederef
-                                (Etempvar _p (tptr (Tstruct _tree noattr)))
-                                (Tstruct _tree noattr)) _key tint))
-                          (Ssequence
-                            (Sset _t'7
-                              (Efield
-                                (Ederef
-                                  (Etempvar _p (tptr (Tstruct _tree noattr)))
-                                  (Tstruct _tree noattr)) _value
-                                (tptr tvoid)))
-                            (Scall None
-                              (Evar _printf (Tfunction
-                                              (Tcons (tptr tschar) Tnil) tint
-                                              {|cc_vararg:=(Some 1); cc_unproto:=false; cc_structret:=false|}))
-                              ((Evar ___stringlit_1 (tarray tschar 15)) ::
-                               (Etempvar _t'6 tint) ::
-                               (Etempvar _t'7 (tptr tvoid)) :: nil))))
-                        (Ssequence
-                          (Scall None
-                            (Evar _release2 (Tfunction
-                                              (Tcons (tptr tvoid) Tnil) tvoid
-                                              cc_default))
-                            ((Etempvar _l (tptr tvoid)) :: nil))
-                          (Sreturn None))))))))))
-        Sskip))))
 |}.
 
 Definition f_findnext := {|
@@ -890,9 +510,9 @@ Definition f_traverse := {|
   fn_vars := nil;
   fn_temps := ((_flag, tint) :: (_b, tint) :: (_t'1, tint) ::
                (_t'8, (tptr (Tstruct _tree_t noattr))) ::
-               (_t'7, (tptr (tarray (tptr tvoid) 2))) ::
+               (_t'7, (tptr (Tstruct _atom_int noattr))) ::
                (_t'6, (tptr (Tstruct _tree_t noattr))) ::
-               (_t'5, (tptr (tarray (tptr tvoid) 2))) ::
+               (_t'5, (tptr (Tstruct _atom_int noattr))) ::
                (_t'4, (tptr (Tstruct _tree_t noattr))) ::
                (_t'3, (tptr (Tstruct _tree noattr))) ::
                (_t'2, (tptr (Tstruct _tree_t noattr))) :: nil);
@@ -961,12 +581,13 @@ Definition f_traverse := {|
                               (Ederef
                                 (Etempvar _t'6 (tptr (Tstruct _tree_t noattr)))
                                 (Tstruct _tree_t noattr)) _lock
-                              (tptr (tarray (tptr tvoid) 2))))
+                              (tptr (Tstruct _atom_int noattr))))
                           (Scall None
                             (Evar _acquire (Tfunction
-                                             (Tcons (tptr tvoid) Tnil) tvoid
-                                             cc_default))
-                            ((Etempvar _t'7 (tptr (tarray (tptr tvoid) 2))) ::
+                                             (Tcons
+                                               (tptr (Tstruct _atom_int noattr))
+                                               Tnil) tvoid cc_default))
+                            ((Etempvar _t'7 (tptr (Tstruct _atom_int noattr))) ::
                              nil))))
                       (Ssequence
                         (Sset _t'4
@@ -981,12 +602,13 @@ Definition f_traverse := {|
                               (Ederef
                                 (Etempvar _t'4 (tptr (Tstruct _tree_t noattr)))
                                 (Tstruct _tree_t noattr)) _lock
-                              (tptr (tarray (tptr tvoid) 2))))
+                              (tptr (Tstruct _atom_int noattr))))
                           (Scall None
-                            (Evar _release2 (Tfunction
-                                              (Tcons (tptr tvoid) Tnil) tvoid
-                                              cc_default))
-                            ((Etempvar _t'5 (tptr (tarray (tptr tvoid) 2))) ::
+                            (Evar _release (Tfunction
+                                             (Tcons
+                                               (tptr (Tstruct _atom_int noattr))
+                                               Tnil) tvoid cc_default))
+                            ((Etempvar _t'5 (tptr (Tstruct _atom_int noattr))) ::
                              nil))))))))))))
       Sskip)
     (Sreturn (Some (Etempvar _flag tint)))))
@@ -1000,11 +622,12 @@ Definition f_insertOp := {|
   fn_vars := nil;
   fn_temps := ((_p1, (tptr (Tstruct _tree_t noattr))) ::
                (_p2, (tptr (Tstruct _tree_t noattr))) ::
-               (_l1, (tptr (tarray (tptr tvoid) 2))) ::
-               (_l2, (tptr (tarray (tptr tvoid) 2))) ::
-               (_t'5, (tptr tvoid)) :: (_t'4, (tptr tvoid)) ::
-               (_t'3, (tptr tvoid)) :: (_t'2, (tptr tvoid)) ::
-               (_t'1, (tptr tvoid)) ::
+               (_l1, (tptr (Tstruct _atom_int noattr))) ::
+               (_l2, (tptr (Tstruct _atom_int noattr))) ::
+               (_t'5, (tptr tvoid)) ::
+               (_t'4, (tptr (Tstruct _atom_int noattr))) ::
+               (_t'3, (tptr (Tstruct _atom_int noattr))) ::
+               (_t'2, (tptr tvoid)) :: (_t'1, (tptr tvoid)) ::
                (_t'14, (tptr (Tstruct _tree_t noattr))) ::
                (_t'13, (tptr (Tstruct _tree noattr))) ::
                (_t'12, (tptr (Tstruct _tree_t noattr))) ::
@@ -1046,167 +669,153 @@ Definition f_insertOp := {|
         (Ssequence
           (Ssequence
             (Scall (Some _t'3)
-              (Evar _surely_malloc (Tfunction (Tcons tulong Tnil)
-                                     (tptr tvoid) cc_default))
-              ((Esizeof (tarray (tptr tvoid) 2) tulong) :: nil))
-            (Sset _l1
-              (Ecast (Etempvar _t'3 (tptr tvoid))
-                (tptr (tarray (tptr tvoid) 2)))))
+              (Evar _makelock (Tfunction Tnil
+                                (tptr (Tstruct _atom_int noattr)) cc_default))
+              nil)
+            (Sset _l1 (Etempvar _t'3 (tptr (Tstruct _atom_int noattr)))))
           (Ssequence
-            (Scall None
-              (Evar _makelock (Tfunction (Tcons (tptr tvoid) Tnil) tvoid
-                                cc_default))
-              ((Etempvar _l1 (tptr (tarray (tptr tvoid) 2))) :: nil))
+            (Sassign
+              (Efield
+                (Ederef (Etempvar _p1 (tptr (Tstruct _tree_t noattr)))
+                  (Tstruct _tree_t noattr)) _lock
+                (tptr (Tstruct _atom_int noattr)))
+              (Etempvar _l1 (tptr (Tstruct _atom_int noattr))))
             (Ssequence
-              (Sassign
-                (Efield
-                  (Ederef (Etempvar _p1 (tptr (Tstruct _tree_t noattr)))
-                    (Tstruct _tree_t noattr)) _lock
-                  (tptr (tarray (tptr tvoid) 2)))
-                (Etempvar _l1 (tptr (tarray (tptr tvoid) 2))))
+              (Scall None
+                (Evar _release (Tfunction
+                                 (Tcons (tptr (Tstruct _atom_int noattr))
+                                   Tnil) tvoid cc_default))
+                ((Etempvar _l1 (tptr (Tstruct _atom_int noattr))) :: nil))
               (Ssequence
-                (Scall None
-                  (Evar _release2 (Tfunction (Tcons (tptr tvoid) Tnil) tvoid
-                                    cc_default))
-                  ((Etempvar _l1 (tptr (tarray (tptr tvoid) 2))) :: nil))
                 (Ssequence
-                  (Ssequence
-                    (Scall (Some _t'4)
-                      (Evar _surely_malloc (Tfunction (Tcons tulong Tnil)
-                                             (tptr tvoid) cc_default))
-                      ((Esizeof (tarray (tptr tvoid) 2) tulong) :: nil))
-                    (Sset _l2
-                      (Ecast (Etempvar _t'4 (tptr tvoid))
-                        (tptr (tarray (tptr tvoid) 2)))))
+                  (Scall (Some _t'4)
+                    (Evar _makelock (Tfunction Tnil
+                                      (tptr (Tstruct _atom_int noattr))
+                                      cc_default)) nil)
+                  (Sset _l2
+                    (Etempvar _t'4 (tptr (Tstruct _atom_int noattr)))))
+                (Ssequence
+                  (Sassign
+                    (Efield
+                      (Ederef (Etempvar _p2 (tptr (Tstruct _tree_t noattr)))
+                        (Tstruct _tree_t noattr)) _lock
+                      (tptr (Tstruct _atom_int noattr)))
+                    (Etempvar _l2 (tptr (Tstruct _atom_int noattr))))
                   (Ssequence
                     (Scall None
-                      (Evar _makelock (Tfunction (Tcons (tptr tvoid) Tnil)
-                                        tvoid cc_default))
-                      ((Etempvar _l2 (tptr (tarray (tptr tvoid) 2))) :: nil))
+                      (Evar _release (Tfunction
+                                       (Tcons
+                                         (tptr (Tstruct _atom_int noattr))
+                                         Tnil) tvoid cc_default))
+                      ((Etempvar _l2 (tptr (Tstruct _atom_int noattr))) ::
+                       nil))
                     (Ssequence
-                      (Sassign
-                        (Efield
-                          (Ederef
-                            (Etempvar _p2 (tptr (Tstruct _tree_t noattr)))
-                            (Tstruct _tree_t noattr)) _lock
-                          (tptr (tarray (tptr tvoid) 2)))
-                        (Etempvar _l2 (tptr (tarray (tptr tvoid) 2))))
                       (Ssequence
-                        (Scall None
-                          (Evar _release2 (Tfunction
-                                            (Tcons (tptr tvoid) Tnil) tvoid
-                                            cc_default))
-                          ((Etempvar _l2 (tptr (tarray (tptr tvoid) 2))) ::
-                           nil))
+                        (Scall (Some _t'5)
+                          (Evar _surely_malloc (Tfunction (Tcons tulong Tnil)
+                                                 (tptr tvoid) cc_default))
+                          ((Esizeof (Tstruct _tree noattr) tulong) :: nil))
+                        (Ssequence
+                          (Sset _t'14
+                            (Efield
+                              (Ederef
+                                (Etempvar _pn__2 (tptr (Tstruct _pn noattr)))
+                                (Tstruct _pn noattr)) _p
+                              (tptr (Tstruct _tree_t noattr))))
+                          (Sassign
+                            (Efield
+                              (Ederef
+                                (Etempvar _t'14 (tptr (Tstruct _tree_t noattr)))
+                                (Tstruct _tree_t noattr)) _t
+                              (tptr (Tstruct _tree noattr)))
+                            (Ecast (Etempvar _t'5 (tptr tvoid))
+                              (tptr (Tstruct _tree noattr))))))
+                      (Ssequence
+                        (Ssequence
+                          (Sset _t'12
+                            (Efield
+                              (Ederef
+                                (Etempvar _pn__2 (tptr (Tstruct _pn noattr)))
+                                (Tstruct _pn noattr)) _p
+                              (tptr (Tstruct _tree_t noattr))))
+                          (Ssequence
+                            (Sset _t'13
+                              (Efield
+                                (Ederef
+                                  (Etempvar _t'12 (tptr (Tstruct _tree_t noattr)))
+                                  (Tstruct _tree_t noattr)) _t
+                                (tptr (Tstruct _tree noattr))))
+                            (Sassign
+                              (Efield
+                                (Ederef
+                                  (Etempvar _t'13 (tptr (Tstruct _tree noattr)))
+                                  (Tstruct _tree noattr)) _key tint)
+                              (Etempvar _x tint))))
                         (Ssequence
                           (Ssequence
-                            (Scall (Some _t'5)
-                              (Evar _surely_malloc (Tfunction
-                                                     (Tcons tulong Tnil)
-                                                     (tptr tvoid) cc_default))
-                              ((Esizeof (Tstruct _tree noattr) tulong) ::
-                               nil))
+                            (Sset _t'10
+                              (Efield
+                                (Ederef
+                                  (Etempvar _pn__2 (tptr (Tstruct _pn noattr)))
+                                  (Tstruct _pn noattr)) _p
+                                (tptr (Tstruct _tree_t noattr))))
                             (Ssequence
-                              (Sset _t'14
+                              (Sset _t'11
                                 (Efield
                                   (Ederef
-                                    (Etempvar _pn__2 (tptr (Tstruct _pn noattr)))
-                                    (Tstruct _pn noattr)) _p
-                                  (tptr (Tstruct _tree_t noattr))))
+                                    (Etempvar _t'10 (tptr (Tstruct _tree_t noattr)))
+                                    (Tstruct _tree_t noattr)) _t
+                                  (tptr (Tstruct _tree noattr))))
                               (Sassign
                                 (Efield
                                   (Ederef
-                                    (Etempvar _t'14 (tptr (Tstruct _tree_t noattr)))
-                                    (Tstruct _tree_t noattr)) _t
-                                  (tptr (Tstruct _tree noattr)))
-                                (Ecast (Etempvar _t'5 (tptr tvoid))
-                                  (tptr (Tstruct _tree noattr))))))
+                                    (Etempvar _t'11 (tptr (Tstruct _tree noattr)))
+                                    (Tstruct _tree noattr)) _value
+                                  (tptr tvoid))
+                                (Etempvar _value (tptr tvoid)))))
                           (Ssequence
                             (Ssequence
-                              (Sset _t'12
+                              (Sset _t'8
                                 (Efield
                                   (Ederef
                                     (Etempvar _pn__2 (tptr (Tstruct _pn noattr)))
                                     (Tstruct _pn noattr)) _p
                                   (tptr (Tstruct _tree_t noattr))))
                               (Ssequence
-                                (Sset _t'13
+                                (Sset _t'9
                                   (Efield
                                     (Ederef
-                                      (Etempvar _t'12 (tptr (Tstruct _tree_t noattr)))
+                                      (Etempvar _t'8 (tptr (Tstruct _tree_t noattr)))
                                       (Tstruct _tree_t noattr)) _t
                                     (tptr (Tstruct _tree noattr))))
                                 (Sassign
                                   (Efield
                                     (Ederef
-                                      (Etempvar _t'13 (tptr (Tstruct _tree noattr)))
-                                      (Tstruct _tree noattr)) _key tint)
-                                  (Etempvar _x tint))))
+                                      (Etempvar _t'9 (tptr (Tstruct _tree noattr)))
+                                      (Tstruct _tree noattr)) _left
+                                    (tptr (Tstruct _tree_t noattr)))
+                                  (Etempvar _p1 (tptr (Tstruct _tree_t noattr))))))
                             (Ssequence
+                              (Sset _t'6
+                                (Efield
+                                  (Ederef
+                                    (Etempvar _pn__2 (tptr (Tstruct _pn noattr)))
+                                    (Tstruct _pn noattr)) _p
+                                  (tptr (Tstruct _tree_t noattr))))
                               (Ssequence
-                                (Sset _t'10
+                                (Sset _t'7
                                   (Efield
                                     (Ederef
-                                      (Etempvar _pn__2 (tptr (Tstruct _pn noattr)))
-                                      (Tstruct _pn noattr)) _p
-                                    (tptr (Tstruct _tree_t noattr))))
-                                (Ssequence
-                                  (Sset _t'11
-                                    (Efield
-                                      (Ederef
-                                        (Etempvar _t'10 (tptr (Tstruct _tree_t noattr)))
-                                        (Tstruct _tree_t noattr)) _t
-                                      (tptr (Tstruct _tree noattr))))
-                                  (Sassign
-                                    (Efield
-                                      (Ederef
-                                        (Etempvar _t'11 (tptr (Tstruct _tree noattr)))
-                                        (Tstruct _tree noattr)) _value
-                                      (tptr tvoid))
-                                    (Etempvar _value (tptr tvoid)))))
-                              (Ssequence
-                                (Ssequence
-                                  (Sset _t'8
-                                    (Efield
-                                      (Ederef
-                                        (Etempvar _pn__2 (tptr (Tstruct _pn noattr)))
-                                        (Tstruct _pn noattr)) _p
-                                      (tptr (Tstruct _tree_t noattr))))
-                                  (Ssequence
-                                    (Sset _t'9
-                                      (Efield
-                                        (Ederef
-                                          (Etempvar _t'8 (tptr (Tstruct _tree_t noattr)))
-                                          (Tstruct _tree_t noattr)) _t
-                                        (tptr (Tstruct _tree noattr))))
-                                    (Sassign
-                                      (Efield
-                                        (Ederef
-                                          (Etempvar _t'9 (tptr (Tstruct _tree noattr)))
-                                          (Tstruct _tree noattr)) _left
-                                        (tptr (Tstruct _tree_t noattr)))
-                                      (Etempvar _p1 (tptr (Tstruct _tree_t noattr))))))
-                                (Ssequence
-                                  (Sset _t'6
-                                    (Efield
-                                      (Ederef
-                                        (Etempvar _pn__2 (tptr (Tstruct _pn noattr)))
-                                        (Tstruct _pn noattr)) _p
-                                      (tptr (Tstruct _tree_t noattr))))
-                                  (Ssequence
-                                    (Sset _t'7
-                                      (Efield
-                                        (Ederef
-                                          (Etempvar _t'6 (tptr (Tstruct _tree_t noattr)))
-                                          (Tstruct _tree_t noattr)) _t
-                                        (tptr (Tstruct _tree noattr))))
-                                    (Sassign
-                                      (Efield
-                                        (Ederef
-                                          (Etempvar _t'7 (tptr (Tstruct _tree noattr)))
-                                          (Tstruct _tree noattr)) _right
-                                        (tptr (Tstruct _tree_t noattr)))
-                                      (Etempvar _p2 (tptr (Tstruct _tree_t noattr))))))))))))))))))))))
+                                      (Etempvar _t'6 (tptr (Tstruct _tree_t noattr)))
+                                      (Tstruct _tree_t noattr)) _t
+                                    (tptr (Tstruct _tree noattr))))
+                                (Sassign
+                                  (Efield
+                                    (Ederef
+                                      (Etempvar _t'7 (tptr (Tstruct _tree noattr)))
+                                      (Tstruct _tree noattr)) _right
+                                    (tptr (Tstruct _tree_t noattr)))
+                                  (Etempvar _p2 (tptr (Tstruct _tree_t noattr))))))))))))))))))))
 |}.
 
 Definition f_insert2 := {|
@@ -1218,11 +827,11 @@ Definition f_insert2 := {|
   fn_temps := ((_pn__2, (tptr (Tstruct _pn noattr))) :: (_t'2, tint) ::
                (_t'1, (tptr tvoid)) ::
                (_t'9, (tptr (Tstruct _tree_t noattr))) ::
-               (_t'8, (tptr (tarray (tptr tvoid) 2))) ::
+               (_t'8, (tptr (Tstruct _atom_int noattr))) ::
                (_t'7, (tptr (Tstruct _tree_t noattr))) ::
                (_t'6, (tptr (Tstruct _tree noattr))) ::
                (_t'5, (tptr (Tstruct _tree_t noattr))) ::
-               (_t'4, (tptr (tarray (tptr tvoid) 2))) ::
+               (_t'4, (tptr (Tstruct _atom_int noattr))) ::
                (_t'3, (tptr (Tstruct _tree_t noattr))) :: nil);
   fn_body :=
 (Ssequence
@@ -1254,11 +863,12 @@ Definition f_insert2 := {|
             (Efield
               (Ederef (Etempvar _t'7 (tptr (Tstruct _tree_t noattr)))
                 (Tstruct _tree_t noattr)) _lock
-              (tptr (tarray (tptr tvoid) 2))))
+              (tptr (Tstruct _atom_int noattr))))
           (Scall None
-            (Evar _acquire (Tfunction (Tcons (tptr tvoid) Tnil) tvoid
-                             cc_default))
-            ((Etempvar _t'8 (tptr (tarray (tptr tvoid) 2))) :: nil))))
+            (Evar _acquire (Tfunction
+                             (Tcons (tptr (Tstruct _atom_int noattr)) Tnil)
+                             tvoid cc_default))
+            ((Etempvar _t'8 (tptr (Tstruct _atom_int noattr))) :: nil))))
       (Ssequence
         (Ssequence
           (Scall (Some _t'2)
@@ -1304,11 +914,12 @@ Definition f_insert2 := {|
                 (Efield
                   (Ederef (Etempvar _t'3 (tptr (Tstruct _tree_t noattr)))
                     (Tstruct _tree_t noattr)) _lock
-                  (tptr (tarray (tptr tvoid) 2))))
+                  (tptr (Tstruct _atom_int noattr))))
               (Scall None
-                (Evar _release2 (Tfunction (Tcons (tptr tvoid) Tnil) tvoid
-                                  cc_default))
-                ((Etempvar _t'4 (tptr (tarray (tptr tvoid) 2))) :: nil))))
+                (Evar _release (Tfunction
+                                 (Tcons (tptr (Tstruct _atom_int noattr))
+                                   Tnil) tvoid cc_default))
+                ((Etempvar _t'4 (tptr (Tstruct _atom_int noattr))) :: nil))))
           (Scall None
             (Evar _free (Tfunction (Tcons (tptr tvoid) Tnil) tvoid
                           cc_default))
@@ -1378,7 +989,7 @@ Definition f_Inorder := {|
                 (Scall None
                   (Evar _printf (Tfunction (Tcons (tptr tschar) Tnil) tint
                                   {|cc_vararg:=(Some 1); cc_unproto:=false; cc_structret:=false|}))
-                  ((Evar ___stringlit_4 (tarray tschar 19)) ::
+                  ((Evar ___stringlit_1 (tarray tschar 19)) ::
                    (Etempvar _t'5 tint) :: (Etempvar _t'7 (tptr tvoid)) ::
                    nil))))))
         (Ssequence
@@ -1405,8 +1016,7 @@ Definition f_traverseInorder := {|
   fn_callconv := cc_default;
   fn_params := ((_t, (tptr (tptr (Tstruct _tree_t noattr)))) :: nil);
   fn_vars := nil;
-  fn_temps := ((_p, (tptr (Tstruct _tree noattr))) ::
-               (_tgt, (tptr (Tstruct _tree_t noattr))) :: nil);
+  fn_temps := ((_tgt, (tptr (Tstruct _tree_t noattr))) :: nil);
   fn_body :=
 (Ssequence
   (Sset _tgt
@@ -1437,11 +1047,12 @@ Definition f_lookup := {|
     (Sset _l
       (Efield
         (Ederef (Etempvar _tgt (tptr (Tstruct _tree_t noattr)))
-          (Tstruct _tree_t noattr)) _lock (tptr (tarray (tptr tvoid) 2))))
+          (Tstruct _tree_t noattr)) _lock (tptr (Tstruct _atom_int noattr))))
     (Ssequence
       (Scall None
-        (Evar _acquire (Tfunction (Tcons (tptr tvoid) Tnil) tvoid cc_default))
-        ((Etempvar _l (tptr tvoid)) :: nil))
+        (Evar _acquire (Tfunction
+                         (Tcons (tptr (Tstruct _atom_int noattr)) Tnil) tvoid
+                         cc_default)) ((Etempvar _l (tptr tvoid)) :: nil))
       (Ssequence
         (Sset _p
           (Efield
@@ -1472,11 +1083,13 @@ Definition f_lookup := {|
                           (Ederef
                             (Etempvar _tgt (tptr (Tstruct _tree_t noattr)))
                             (Tstruct _tree_t noattr)) _lock
-                          (tptr (tarray (tptr tvoid) 2))))
+                          (tptr (Tstruct _atom_int noattr))))
                       (Ssequence
                         (Scall None
-                          (Evar _acquire (Tfunction (Tcons (tptr tvoid) Tnil)
-                                           tvoid cc_default))
+                          (Evar _acquire (Tfunction
+                                           (Tcons
+                                             (tptr (Tstruct _atom_int noattr))
+                                             Tnil) tvoid cc_default))
                           ((Etempvar _l (tptr tvoid)) :: nil))
                         (Ssequence
                           (Sset _p
@@ -1486,9 +1099,10 @@ Definition f_lookup := {|
                                 (Tstruct _tree_t noattr)) _t
                               (tptr (Tstruct _tree noattr))))
                           (Scall None
-                            (Evar _release2 (Tfunction
-                                              (Tcons (tptr tvoid) Tnil) tvoid
-                                              cc_default))
+                            (Evar _release (Tfunction
+                                             (Tcons
+                                               (tptr (Tstruct _atom_int noattr))
+                                               Tnil) tvoid cc_default))
                             ((Etempvar _l_old (tptr tvoid)) :: nil)))))))
                 (Sifthenelse (Ebinop Olt (Etempvar _y tint)
                                (Etempvar _x tint) tint)
@@ -1506,12 +1120,13 @@ Definition f_lookup := {|
                             (Ederef
                               (Etempvar _tgt (tptr (Tstruct _tree_t noattr)))
                               (Tstruct _tree_t noattr)) _lock
-                            (tptr (tarray (tptr tvoid) 2))))
+                            (tptr (Tstruct _atom_int noattr))))
                         (Ssequence
                           (Scall None
                             (Evar _acquire (Tfunction
-                                             (Tcons (tptr tvoid) Tnil) tvoid
-                                             cc_default))
+                                             (Tcons
+                                               (tptr (Tstruct _atom_int noattr))
+                                               Tnil) tvoid cc_default))
                             ((Etempvar _l (tptr tvoid)) :: nil))
                           (Ssequence
                             (Sset _p
@@ -1521,9 +1136,10 @@ Definition f_lookup := {|
                                   (Tstruct _tree_t noattr)) _t
                                 (tptr (Tstruct _tree noattr))))
                             (Scall None
-                              (Evar _release2 (Tfunction
-                                                (Tcons (tptr tvoid) Tnil)
-                                                tvoid cc_default))
+                              (Evar _release (Tfunction
+                                               (Tcons
+                                                 (tptr (Tstruct _atom_int noattr))
+                                                 Tnil) tvoid cc_default))
                               ((Etempvar _l_old__1 (tptr tvoid)) :: nil)))))))
                   (Ssequence
                     (Sset _v
@@ -1532,14 +1148,17 @@ Definition f_lookup := {|
                           (Tstruct _tree noattr)) _value (tptr tvoid)))
                     (Ssequence
                       (Scall None
-                        (Evar _release2 (Tfunction (Tcons (tptr tvoid) Tnil)
-                                          tvoid cc_default))
+                        (Evar _release (Tfunction
+                                         (Tcons
+                                           (tptr (Tstruct _atom_int noattr))
+                                           Tnil) tvoid cc_default))
                         ((Etempvar _l (tptr tvoid)) :: nil))
                       (Sreturn (Some (Etempvar _v (tptr tvoid))))))))))
           (Ssequence
             (Scall None
-              (Evar _release2 (Tfunction (Tcons (tptr tvoid) Tnil) tvoid
-                                cc_default))
+              (Evar _release (Tfunction
+                               (Tcons (tptr (Tstruct _atom_int noattr)) Tnil)
+                               tvoid cc_default))
               ((Etempvar _l (tptr tvoid)) :: nil))
             (Sreturn (Some (Ecast (Econst_int (Int.repr 0) tint)
                              (tptr tvoid))))))))))
@@ -1550,19 +1169,45 @@ Definition f_thread_func := {|
   fn_callconv := cc_default;
   fn_params := ((_args, (tptr tvoid)) :: nil);
   fn_vars := nil;
-  fn_temps := ((_l, (tptr (tarray (tptr tvoid) 2))) :: nil);
+  fn_temps := ((_l, (tptr (Tstruct _atom_int noattr))) ::
+               (_t'2, (tptr (tptr (Tstruct _tree_t noattr)))) ::
+               (_t'1, (tptr (tptr (Tstruct _tree_t noattr)))) :: nil);
   fn_body :=
 (Ssequence
   (Sset _l
-    (Eaddrof (Evar _thread_lock (tarray (tptr tvoid) 2))
-      (tptr (tarray (tptr tvoid) 2))))
+    (Ecast (Etempvar _args (tptr tvoid)) (tptr (Tstruct _atom_int noattr))))
   (Ssequence
-    (Scall None
-      (Evar _release2 (Tfunction (Tcons (tptr tvoid) Tnil) tvoid cc_default))
-      ((Ecast (Etempvar _l (tptr (tarray (tptr tvoid) 2))) (tptr tvoid)) ::
-       nil))
-    (Sreturn (Some (Ecast (Ecast (Econst_int (Int.repr 0) tint) (tptr tvoid))
-                     (tptr tvoid))))))
+    (Ssequence
+      (Sset _t'2 (Evar _tb (tptr (tptr (Tstruct _tree_t noattr)))))
+      (Scall None
+        (Evar _insert2 (Tfunction
+                         (Tcons (tptr (tptr (Tstruct _tree_t noattr)))
+                           (Tcons tint (Tcons (tptr tvoid) Tnil))) tvoid
+                         cc_default))
+        ((Etempvar _t'2 (tptr (tptr (Tstruct _tree_t noattr)))) ::
+         (Econst_int (Int.repr 6) tint) ::
+         (Evar ___stringlit_2 (tarray tschar 16)) :: nil)))
+    (Ssequence
+      (Ssequence
+        (Sset _t'1 (Evar _tb (tptr (tptr (Tstruct _tree_t noattr)))))
+        (Scall None
+          (Evar _insert2 (Tfunction
+                           (Tcons (tptr (tptr (Tstruct _tree_t noattr)))
+                             (Tcons tint (Tcons (tptr tvoid) Tnil))) tvoid
+                           cc_default))
+          ((Etempvar _t'1 (tptr (tptr (Tstruct _tree_t noattr)))) ::
+           (Econst_int (Int.repr 4) tint) ::
+           (Evar ___stringlit_3 (tarray tschar 5)) :: nil)))
+      (Ssequence
+        (Scall None
+          (Evar _release (Tfunction
+                           (Tcons (tptr (Tstruct _atom_int noattr)) Tnil)
+                           tvoid cc_default))
+          ((Ecast (Etempvar _l (tptr (Tstruct _atom_int noattr)))
+             (tptr tvoid)) :: nil))
+        (Sreturn (Some (Ecast
+                         (Ecast (Econst_int (Int.repr 0) tint) (tptr tvoid))
+                         (tptr tvoid))))))))
 |}.
 
 Definition f_main := {|
@@ -1570,15 +1215,16 @@ Definition f_main := {|
   fn_callconv := cc_default;
   fn_params := nil;
   fn_vars := nil;
-  fn_temps := ((_t_lock, (tptr (tarray (tptr tvoid) 2))) ::
-               (_t'2, (tptr tvoid)) ::
+  fn_temps := ((_t_lock, (tptr (Tstruct _atom_int noattr))) ::
+               (_t'3, (tptr tvoid)) ::
+               (_t'2, (tptr (Tstruct _atom_int noattr))) ::
                (_t'1, (tptr (tptr (Tstruct _tree_t noattr)))) ::
+               (_t'9, (tptr (tptr (Tstruct _tree_t noattr)))) ::
                (_t'8, (tptr (tptr (Tstruct _tree_t noattr)))) ::
                (_t'7, (tptr (tptr (Tstruct _tree_t noattr)))) ::
                (_t'6, (tptr (tptr (Tstruct _tree_t noattr)))) ::
                (_t'5, (tptr (tptr (Tstruct _tree_t noattr)))) ::
-               (_t'4, (tptr (tptr (Tstruct _tree_t noattr)))) ::
-               (_t'3, (tptr (tptr (Tstruct _tree_t noattr)))) :: nil);
+               (_t'4, (tptr (tptr (Tstruct _tree_t noattr)))) :: nil);
   fn_body :=
 (Ssequence
   (Ssequence
@@ -1590,9 +1236,16 @@ Definition f_main := {|
       (Sassign (Evar _tb (tptr (tptr (Tstruct _tree_t noattr))))
         (Etempvar _t'1 (tptr (tptr (Tstruct _tree_t noattr))))))
     (Ssequence
-      (Sset _t_lock
-        (Eaddrof (Evar _thread_lock (tarray (tptr tvoid) 2))
-          (tptr (tarray (tptr tvoid) 2))))
+      (Ssequence
+        (Sset _t'9 (Evar _tb (tptr (tptr (Tstruct _tree_t noattr)))))
+        (Scall None
+          (Evar _insert2 (Tfunction
+                           (Tcons (tptr (tptr (Tstruct _tree_t noattr)))
+                             (Tcons tint (Tcons (tptr tvoid) Tnil))) tvoid
+                           cc_default))
+          ((Etempvar _t'9 (tptr (tptr (Tstruct _tree_t noattr)))) ::
+           (Econst_int (Int.repr 3) tint) ::
+           (Evar ___stringlit_4 (tarray tschar 6)) :: nil)))
       (Ssequence
         (Ssequence
           (Sset _t'8 (Evar _tb (tptr (tptr (Tstruct _tree_t noattr)))))
@@ -1602,8 +1255,8 @@ Definition f_main := {|
                                (Tcons tint (Tcons (tptr tvoid) Tnil))) tvoid
                              cc_default))
             ((Etempvar _t'8 (tptr (tptr (Tstruct _tree_t noattr)))) ::
-             (Econst_int (Int.repr 3) tint) ::
-             (Evar ___stringlit_5 (tarray tschar 6)) :: nil)))
+             (Econst_int (Int.repr 1) tint) ::
+             (Evar ___stringlit_5 (tarray tschar 4)) :: nil)))
         (Ssequence
           (Ssequence
             (Sset _t'7 (Evar _tb (tptr (tptr (Tstruct _tree_t noattr)))))
@@ -1613,106 +1266,97 @@ Definition f_main := {|
                                  (Tcons tint (Tcons (tptr tvoid) Tnil)))
                                tvoid cc_default))
               ((Etempvar _t'7 (tptr (tptr (Tstruct _tree_t noattr)))) ::
-               (Econst_int (Int.repr 1) tint) ::
-               (Evar ___stringlit_6 (tarray tschar 4)) :: nil)))
+               (Econst_int (Int.repr 4) tint) ::
+               (Evar ___stringlit_6 (tarray tschar 5)) :: nil)))
           (Ssequence
             (Ssequence
-              (Sset _t'6 (Evar _tb (tptr (tptr (Tstruct _tree_t noattr)))))
-              (Scall None
-                (Evar _insert2 (Tfunction
-                                 (Tcons
-                                   (tptr (tptr (Tstruct _tree_t noattr)))
-                                   (Tcons tint (Tcons (tptr tvoid) Tnil)))
-                                 tvoid cc_default))
-                ((Etempvar _t'6 (tptr (tptr (Tstruct _tree_t noattr)))) ::
-                 (Econst_int (Int.repr 4) tint) ::
-                 (Evar ___stringlit_7 (tarray tschar 5)) :: nil)))
+              (Scall (Some _t'2)
+                (Evar _makelock (Tfunction Tnil
+                                  (tptr (Tstruct _atom_int noattr))
+                                  cc_default)) nil)
+              (Sset _t_lock
+                (Etempvar _t'2 (tptr (Tstruct _atom_int noattr)))))
             (Ssequence
               (Scall None
-                (Evar _makelock (Tfunction (Tcons (tptr tvoid) Tnil) tvoid
-                                  cc_default))
-                ((Ecast (Etempvar _t_lock (tptr (tarray (tptr tvoid) 2)))
+                (Evar _spawn (Tfunction
+                               (Tcons
+                                 (tptr (Tfunction (Tcons (tptr tvoid) Tnil)
+                                         tint cc_default))
+                                 (Tcons (tptr tvoid) Tnil)) tvoid cc_default))
+                ((Ecast
+                   (Eaddrof
+                     (Evar _thread_func (Tfunction (Tcons (tptr tvoid) Tnil)
+                                          (tptr tvoid) cc_default))
+                     (tptr (Tfunction (Tcons (tptr tvoid) Tnil) (tptr tvoid)
+                             cc_default))) (tptr tvoid)) ::
+                 (Ecast (Etempvar _t_lock (tptr (Tstruct _atom_int noattr)))
                    (tptr tvoid)) :: nil))
               (Ssequence
                 (Scall None
-                  (Evar _spawn (Tfunction
-                                 (Tcons
-                                   (tptr (Tfunction (Tcons (tptr tvoid) Tnil)
-                                           (tptr tvoid) cc_default))
-                                   (Tcons (tptr tvoid) Tnil)) tvoid
-                                 cc_default))
+                  (Evar _acquire (Tfunction
+                                   (Tcons (tptr (Tstruct _atom_int noattr))
+                                     Tnil) tvoid cc_default))
                   ((Ecast
-                     (Eaddrof
-                       (Evar _thread_func (Tfunction
-                                            (Tcons (tptr tvoid) Tnil)
-                                            (tptr tvoid) cc_default))
-                       (tptr (Tfunction (Tcons (tptr tvoid) Tnil)
-                               (tptr tvoid) cc_default))) (tptr tvoid)) ::
-                   (Ecast (Ecast (Econst_int (Int.repr 0) tint) (tptr tvoid))
+                     (Etempvar _t_lock (tptr (Tstruct _atom_int noattr)))
                      (tptr tvoid)) :: nil))
                 (Ssequence
                   (Scall None
-                    (Evar _acquire (Tfunction (Tcons (tptr tvoid) Tnil) tvoid
-                                     cc_default))
-                    ((Ecast (Etempvar _t_lock (tptr (tarray (tptr tvoid) 2)))
+                    (Evar _freelock (Tfunction
+                                      (Tcons
+                                        (tptr (Tstruct _atom_int noattr))
+                                        Tnil) tvoid cc_default))
+                    ((Ecast
+                       (Etempvar _t_lock (tptr (Tstruct _atom_int noattr)))
                        (tptr tvoid)) :: nil))
                   (Ssequence
-                    (Scall None
-                      (Evar _freelock2 (Tfunction (Tcons (tptr tvoid) Tnil)
-                                         tvoid cc_default))
-                      ((Ecast
-                         (Etempvar _t_lock (tptr (tarray (tptr tvoid) 2)))
-                         (tptr tvoid)) :: nil))
                     (Ssequence
+                      (Ssequence
+                        (Sset _t'6
+                          (Evar _tb (tptr (tptr (Tstruct _tree_t noattr)))))
+                        (Scall (Some _t'3)
+                          (Evar _lookup (Tfunction
+                                          (Tcons
+                                            (tptr (tptr (Tstruct _tree_t noattr)))
+                                            (Tcons tint Tnil)) (tptr tvoid)
+                                          cc_default))
+                          ((Etempvar _t'6 (tptr (tptr (Tstruct _tree_t noattr)))) ::
+                           (Econst_int (Int.repr 4) tint) :: nil)))
+                      (Scall None
+                        (Evar _printf (Tfunction (Tcons (tptr tschar) Tnil)
+                                        tint
+                                        {|cc_vararg:=(Some 1); cc_unproto:=false; cc_structret:=false|}))
+                        ((Evar ___stringlit_7 (tarray tschar 4)) ::
+                         (Etempvar _t'3 (tptr tvoid)) :: nil)))
+                    (Ssequence
+                      (Scall None
+                        (Evar _printf (Tfunction (Tcons (tptr tschar) Tnil)
+                                        tint
+                                        {|cc_vararg:=(Some 1); cc_unproto:=false; cc_structret:=false|}))
+                        ((Evar ___stringlit_8 (tarray tschar 10)) :: nil))
                       (Ssequence
                         (Ssequence
                           (Sset _t'5
                             (Evar _tb (tptr (tptr (Tstruct _tree_t noattr)))))
-                          (Scall (Some _t'2)
-                            (Evar _lookup (Tfunction
-                                            (Tcons
-                                              (tptr (tptr (Tstruct _tree_t noattr)))
-                                              (Tcons tint Tnil)) (tptr tvoid)
-                                            cc_default))
+                          (Scall None
+                            (Evar _traverseInorder (Tfunction
+                                                     (Tcons
+                                                       (tptr (tptr (Tstruct _tree_t noattr)))
+                                                       Tnil) tvoid
+                                                     cc_default))
                             ((Etempvar _t'5 (tptr (tptr (Tstruct _tree_t noattr)))) ::
-                             (Econst_int (Int.repr 4) tint) :: nil)))
-                        (Scall None
-                          (Evar _printf (Tfunction (Tcons (tptr tschar) Tnil)
-                                          tint
-                                          {|cc_vararg:=(Some 1); cc_unproto:=false; cc_structret:=false|}))
-                          ((Evar ___stringlit_8 (tarray tschar 4)) ::
-                           (Etempvar _t'2 (tptr tvoid)) :: nil)))
-                      (Ssequence
-                        (Scall None
-                          (Evar _printf (Tfunction (Tcons (tptr tschar) Tnil)
-                                          tint
-                                          {|cc_vararg:=(Some 1); cc_unproto:=false; cc_structret:=false|}))
-                          ((Evar ___stringlit_9 (tarray tschar 10)) :: nil))
+                             nil)))
                         (Ssequence
                           (Ssequence
                             (Sset _t'4
                               (Evar _tb (tptr (tptr (Tstruct _tree_t noattr)))))
                             (Scall None
-                              (Evar _traverseInorder (Tfunction
-                                                       (Tcons
-                                                         (tptr (tptr (Tstruct _tree_t noattr)))
-                                                         Tnil) tvoid
-                                                       cc_default))
+                              (Evar _treebox_free (Tfunction
+                                                    (Tcons
+                                                      (tptr (tptr (Tstruct _tree_t noattr)))
+                                                      Tnil) tvoid cc_default))
                               ((Etempvar _t'4 (tptr (tptr (Tstruct _tree_t noattr)))) ::
                                nil)))
-                          (Ssequence
-                            (Ssequence
-                              (Sset _t'3
-                                (Evar _tb (tptr (tptr (Tstruct _tree_t noattr)))))
-                              (Scall None
-                                (Evar _treebox_free (Tfunction
-                                                      (Tcons
-                                                        (tptr (tptr (Tstruct _tree_t noattr)))
-                                                        Tnil) tvoid
-                                                      cc_default))
-                                ((Etempvar _t'3 (tptr (tptr (Tstruct _tree_t noattr)))) ::
-                                 nil)))
-                            (Sreturn (Some (Econst_int (Int.repr 0) tint))))))))))))))))
+                          (Sreturn (Some (Econst_int (Int.repr 0) tint)))))))))))))))
   (Sreturn (Some (Econst_int (Int.repr 0) tint))))
 |}.
 
@@ -1724,7 +1368,7 @@ Definition composites : list composite_definition :=
    noattr ::
  Composite _tree_t Struct
    (Member_plain _t (tptr (Tstruct _tree noattr)) ::
-    Member_plain _lock (tptr (tarray (tptr tvoid) 2)) :: nil)
+    Member_plain _lock (tptr (Tstruct _atom_int noattr)) :: nil)
    noattr ::
  Composite _pn Struct
    (Member_plain _p (tptr (Tstruct _tree_t noattr)) ::
@@ -1817,15 +1461,14 @@ Definition global_definitions : list (ident * globdef fundef type) :=
    Gfun(External (EF_runtime "__compcert_i64_umulh"
                    (mksignature (AST.Tlong :: AST.Tlong :: nil) AST.Tlong
                      cc_default)) (Tcons tulong (Tcons tulong Tnil)) tulong
-     cc_default)) :: (___stringlit_7, Gvar v___stringlit_7) ::
- (___stringlit_5, Gvar v___stringlit_5) ::
- (___stringlit_2, Gvar v___stringlit_2) ::
+     cc_default)) :: (___stringlit_6, Gvar v___stringlit_6) ::
  (___stringlit_4, Gvar v___stringlit_4) ::
- (___stringlit_3, Gvar v___stringlit_3) ::
- (___stringlit_9, Gvar v___stringlit_9) ::
  (___stringlit_1, Gvar v___stringlit_1) ::
  (___stringlit_8, Gvar v___stringlit_8) ::
- (___stringlit_6, Gvar v___stringlit_6) ::
+ (___stringlit_2, Gvar v___stringlit_2) ::
+ (___stringlit_7, Gvar v___stringlit_7) ::
+ (___stringlit_5, Gvar v___stringlit_5) ::
+ (___stringlit_3, Gvar v___stringlit_3) ::
  (___builtin_bswap64,
    Gfun(External (EF_builtin "__builtin_bswap64"
                    (mksignature (AST.Tlong :: nil) AST.Tlong cc_default))
@@ -2007,29 +1650,6 @@ Definition global_definitions : list (ident * globdef fundef type) :=
                      {|cc_vararg:=(Some 1); cc_unproto:=false; cc_structret:=false|}))
      (Tcons (tptr tschar) Tnil) tint
      {|cc_vararg:=(Some 1); cc_unproto:=false; cc_structret:=false|})) ::
- (_makelock,
-   Gfun(External (EF_external "makelock"
-                   (mksignature (AST.Tlong :: nil) AST.Tvoid cc_default))
-     (Tcons (tptr tvoid) Tnil) tvoid cc_default)) ::
- (_acquire,
-   Gfun(External (EF_external "acquire"
-                   (mksignature (AST.Tlong :: nil) AST.Tvoid cc_default))
-     (Tcons (tptr tvoid) Tnil) tvoid cc_default)) ::
- (_freelock2,
-   Gfun(External (EF_external "freelock2"
-                   (mksignature (AST.Tlong :: nil) AST.Tvoid cc_default))
-     (Tcons (tptr tvoid) Tnil) tvoid cc_default)) ::
- (_release2,
-   Gfun(External (EF_external "release2"
-                   (mksignature (AST.Tlong :: nil) AST.Tvoid cc_default))
-     (Tcons (tptr tvoid) Tnil) tvoid cc_default)) ::
- (_spawn,
-   Gfun(External (EF_external "spawn"
-                   (mksignature (AST.Tlong :: AST.Tlong :: nil) AST.Tvoid
-                     cc_default))
-     (Tcons
-       (tptr (Tfunction (Tcons (tptr tvoid) Tnil) (tptr tvoid) cc_default))
-       (Tcons (tptr tvoid) Tnil)) tvoid cc_default)) ::
  (_malloc,
    Gfun(External EF_malloc (Tcons tulong Tnil) (tptr tvoid) cc_default)) ::
  (_free, Gfun(External EF_free (Tcons (tptr tvoid) Tnil) tvoid cc_default)) ::
@@ -2037,12 +1657,32 @@ Definition global_definitions : list (ident * globdef fundef type) :=
    Gfun(External (EF_external "exit"
                    (mksignature (AST.Tint :: nil) AST.Tvoid cc_default))
      (Tcons tint Tnil) tvoid cc_default)) ::
- (_thread_lock, Gvar v_thread_lock) :: (_tb, Gvar v_tb) ::
+ (_makelock,
+   Gfun(External (EF_external "makelock"
+                   (mksignature nil AST.Tlong cc_default)) Tnil
+     (tptr (Tstruct _atom_int noattr)) cc_default)) ::
+ (_freelock,
+   Gfun(External (EF_external "freelock"
+                   (mksignature (AST.Tlong :: nil) AST.Tvoid cc_default))
+     (Tcons (tptr (Tstruct _atom_int noattr)) Tnil) tvoid cc_default)) ::
+ (_acquire,
+   Gfun(External (EF_external "acquire"
+                   (mksignature (AST.Tlong :: nil) AST.Tvoid cc_default))
+     (Tcons (tptr (Tstruct _atom_int noattr)) Tnil) tvoid cc_default)) ::
+ (_release,
+   Gfun(External (EF_external "release"
+                   (mksignature (AST.Tlong :: nil) AST.Tvoid cc_default))
+     (Tcons (tptr (Tstruct _atom_int noattr)) Tnil) tvoid cc_default)) ::
+ (_spawn,
+   Gfun(External (EF_external "spawn"
+                   (mksignature (AST.Tlong :: AST.Tlong :: nil) AST.Tvoid
+                     cc_default))
+     (Tcons (tptr (Tfunction (Tcons (tptr tvoid) Tnil) tint cc_default))
+       (Tcons (tptr tvoid) Tnil)) tvoid cc_default)) :: (_tb, Gvar v_tb) ::
  (_surely_malloc, Gfun(Internal f_surely_malloc)) ::
  (_treebox_new, Gfun(Internal f_treebox_new)) ::
  (_tree_free, Gfun(Internal f_tree_free)) ::
  (_treebox_free, Gfun(Internal f_treebox_free)) ::
- (_insert, Gfun(Internal f_insert)) ::
  (_findnext, Gfun(Internal f_findnext)) ::
  (_traverse, Gfun(Internal f_traverse)) ::
  (_insertOp, Gfun(Internal f_insertOp)) ::
@@ -2055,29 +1695,29 @@ Definition global_definitions : list (ident * globdef fundef type) :=
 
 Definition public_idents : list ident :=
 (_main :: _thread_func :: _lookup :: _traverseInorder :: _Inorder ::
- _insert2 :: _insertOp :: _traverse :: _findnext :: _insert ::
- _treebox_free :: _tree_free :: _treebox_new :: _surely_malloc :: _tb ::
- _thread_lock :: _exit :: _free :: _malloc :: _spawn :: _release2 ::
- _freelock2 :: _acquire :: _makelock :: _printf :: ___builtin_debug ::
- ___builtin_write32_reversed :: ___builtin_write16_reversed ::
- ___builtin_read32_reversed :: ___builtin_read16_reversed ::
- ___builtin_fnmsub :: ___builtin_fnmadd :: ___builtin_fmsub ::
- ___builtin_fmadd :: ___builtin_fmin :: ___builtin_fmax ::
- ___builtin_expect :: ___builtin_unreachable :: ___builtin_va_end ::
- ___builtin_va_copy :: ___builtin_va_arg :: ___builtin_va_start ::
- ___builtin_membar :: ___builtin_annot_intval :: ___builtin_annot ::
- ___builtin_sel :: ___builtin_memcpy_aligned :: ___builtin_sqrt ::
- ___builtin_fsqrt :: ___builtin_fabsf :: ___builtin_fabs ::
- ___builtin_ctzll :: ___builtin_ctzl :: ___builtin_ctz :: ___builtin_clzll ::
- ___builtin_clzl :: ___builtin_clz :: ___builtin_bswap16 ::
- ___builtin_bswap32 :: ___builtin_bswap :: ___builtin_bswap64 ::
- ___compcert_i64_umulh :: ___compcert_i64_smulh :: ___compcert_i64_sar ::
- ___compcert_i64_shr :: ___compcert_i64_shl :: ___compcert_i64_umod ::
- ___compcert_i64_smod :: ___compcert_i64_udiv :: ___compcert_i64_sdiv ::
- ___compcert_i64_utof :: ___compcert_i64_stof :: ___compcert_i64_utod ::
- ___compcert_i64_stod :: ___compcert_i64_dtou :: ___compcert_i64_dtos ::
- ___compcert_va_composite :: ___compcert_va_float64 ::
- ___compcert_va_int64 :: ___compcert_va_int32 :: nil).
+ _insert2 :: _insertOp :: _traverse :: _findnext :: _treebox_free ::
+ _tree_free :: _treebox_new :: _surely_malloc :: _tb :: _spawn :: _release ::
+ _acquire :: _freelock :: _makelock :: _exit :: _free :: _malloc ::
+ _printf :: ___builtin_debug :: ___builtin_write32_reversed ::
+ ___builtin_write16_reversed :: ___builtin_read32_reversed ::
+ ___builtin_read16_reversed :: ___builtin_fnmsub :: ___builtin_fnmadd ::
+ ___builtin_fmsub :: ___builtin_fmadd :: ___builtin_fmin ::
+ ___builtin_fmax :: ___builtin_expect :: ___builtin_unreachable ::
+ ___builtin_va_end :: ___builtin_va_copy :: ___builtin_va_arg ::
+ ___builtin_va_start :: ___builtin_membar :: ___builtin_annot_intval ::
+ ___builtin_annot :: ___builtin_sel :: ___builtin_memcpy_aligned ::
+ ___builtin_sqrt :: ___builtin_fsqrt :: ___builtin_fabsf ::
+ ___builtin_fabs :: ___builtin_ctzll :: ___builtin_ctzl :: ___builtin_ctz ::
+ ___builtin_clzll :: ___builtin_clzl :: ___builtin_clz ::
+ ___builtin_bswap16 :: ___builtin_bswap32 :: ___builtin_bswap ::
+ ___builtin_bswap64 :: ___compcert_i64_umulh :: ___compcert_i64_smulh ::
+ ___compcert_i64_sar :: ___compcert_i64_shr :: ___compcert_i64_shl ::
+ ___compcert_i64_umod :: ___compcert_i64_smod :: ___compcert_i64_udiv ::
+ ___compcert_i64_sdiv :: ___compcert_i64_utof :: ___compcert_i64_stof ::
+ ___compcert_i64_utod :: ___compcert_i64_stod :: ___compcert_i64_dtou ::
+ ___compcert_i64_dtos :: ___compcert_va_composite ::
+ ___compcert_va_float64 :: ___compcert_va_int64 :: ___compcert_va_int32 ::
+ nil).
 
 Definition prog : Clight.program := 
   mkprogram composites global_definitions public_idents _main Logic.I.
